operations/Linearize2.thy
@@ -2,16 +2,6 @@ theory Linearize2
   imports "Binders.MRBNF_Composition" "Binders.MRBNF_Recursor"
 begin
 
-(* This theory we start with an MRBNF F, which is assumed (in the imported theory 
-Common_Data_Codata_Bindings) to have the following characteristics:
-  ** is map-constrained to small-support endofunctions in the 1st position, 
-  ** is map-constrained to small-support endobijections in the 2nd position,  
-  ** is unconstrained in the 3rd and 4th position.   
-We show that applying the nonrepetitiveness construction at the 3rd position (on which F is assumed 
-to be pullback-preserving), we transform it into an MRBNF F' that has the same characteristics 
-as F except that the 3rd position becomes map-constrained to small-support endobijections.  
-*)
-
 typedecl ('a, 'b, 'c, 'd, 'e, 'f) F
 consts map_F :: "('a \<Rightarrow> 'a') \<Rightarrow> ('b :: var \<Rightarrow> 'b) \<Rightarrow>
   ('c :: var \<Rightarrow> 'c) \<Rightarrow> ('d \<Rightarrow> 'd') \<Rightarrow> ('e :: var \<Rightarrow> 'e) \<Rightarrow> ('a, 'b, 'c, 'd, 'e, 'f) F \<Rightarrow> ('a', 'b, 'c, 'd', 'e, 'f) F"
@@ -21,6 +11,7 @@ consts set3_F :: "('a, 'b :: var, 'c :: var, 'd, 'e :: var, 'f) F \<Rightarrow> 
 consts set4_F :: "('a, 'b :: var, 'c :: var, 'd, 'e :: var, 'f) F \<Rightarrow> 'd set"
 consts set5_F :: "('a, 'b :: var, 'c :: var, 'd, 'e :: var, 'f) F \<Rightarrow> 'e set"
 consts rrel_F :: "('a \<Rightarrow> 'a' \<Rightarrow> bool) \<Rightarrow> ('d \<Rightarrow> 'd' \<Rightarrow> bool) \<Rightarrow> ('a, 'b :: var, 'c :: var, 'd, 'e::var, 'f) F \<Rightarrow> ('a', 'b, 'c, 'd', 'e, 'f) F \<Rightarrow> bool"
+
 
 declare [[mrbnf_internals]]
 declare [[typedef_overloaded]]
@@ -32,9 +23,8 @@ mrbnf "('a, 'b :: var, 'c :: var, 'd, 'e :: var, 'f) F"
   var_class: var
   sorry
 
-print_mrbnfs
-declare [[ML_print_depth=10000]]
-ML \<open>MRBNF_Def.mrbnf_of @{context} @{type_name F} |> the |> MRBNF_Def.var_types_of_mrbnf\<close>
+(* we linearize this MRBNF on position 1*)
+ML \<open>val lin_pos = 1\<close>
 
 axiomatization where
   (* The next property assumes preservation of pullbacks on the third position. 
@@ -47,23 +37,9 @@ axiomatization where
             set4_F z \<subseteq> {(x, y). S x y} \<and> map_F fst id id fst id z = x \<and> map_F snd id id snd id z = y)"
   and
   (* The next property assumes that nonrepetitive elements exist: *)
-  ex_nonrep: "\<exists>x. \<forall>x'. (\<exists> R. rrel_F (=) R x x') \<longrightarrow> (\<exists> f. x' = map_F f id id id id x)"
+  ex_nonrep: "\<exists>x. \<forall>x'. (\<exists> R. rrel_F R (=) x x') \<longrightarrow> (\<exists> f. x' = map_F f id id id id x)"
 
 abbreviation "rel_F \<equiv> mr_rel_F"
-
-
-(* necessary helper for F_strong *)
-ML \<open>
-open BNF_Util BNF_Tactics
-fun mk_inf_apply_2_set_tac ctxt =
-  HEADGOAL (EVERY' [
-    rtac ctxt @{thm Collect_cong},
-    rtac ctxt @{thm prod.case_cong},
-    rtac ctxt refl,
-    K (unfold_thms_tac ctxt [@{thm inf_apply}]),
-    rtac ctxt refl
-  ])
-\<close>
 
 (* Important consequence of preservation of pullbacks (which is actually equivalent to it): 
 The relator is closed under intersections. *)
@@ -94,11 +70,6 @@ fun mk_F_strong_tac mrbnf F_map_id mr_rel_F_def F_mr_rel_mono_strong0 F_rel_map_
     REPEAT_DETERM_N 7 (HEADGOAL (etac ctxt conjE)) THEN
     HEADGOAL (Subgoal.FOCUS
       (fn {prems, context = ctxt, params, ...} => 
-      let
-        val _ = prems |> map @{print tracing}
-        val _ = params |> map @{print tracing}
-      in
-        print_tac @{context} "SUBGOAL" THEN
         HEADGOAL (Method.insert_tac ctxt [
           infer_instantiate' ctxt [SOME (snd (nth params 1)), SOME (snd (nth params 0))] (@{thm spec2} OF [nth prems 0]),
           infer_instantiate' ctxt [SOME (snd (nth params 2)), SOME (snd (nth params 0))] (@{thm spec2} OF [nth prems 0])] THEN_ALL_NEW
@@ -111,7 +82,6 @@ fun mk_F_strong_tac mrbnf F_map_id mr_rel_F_def F_mr_rel_mono_strong0 F_rel_map_
         HEADGOAL (rtac ctxt exI) THEN
         unfold_thms_tac ctxt @{thms inf_fun_def inf_bool_def} THEN
         HEADGOAL (rtac ctxt conjI) THEN
-  
         HEADGOAL (Method.insert_tac ctxt prems) THEN
         HEADGOAL (hyp_subst_tac_thin true ctxt) THEN
         HEADGOAL (rtac ctxt conjI) THEN
@@ -123,84 +93,76 @@ fun mk_F_strong_tac mrbnf F_map_id mr_rel_F_def F_mr_rel_mono_strong0 F_rel_map_
             etac ctxt (@{thm rev_subsetD} RS (iffD1 OF @{thms prod_in_Collect_iff})),
         assume_tac ctxt,
         assume_tac ctxt])) THEN
-  
         HEADGOAL (rtac ctxt conjI THEN_ALL_NEW resolve_tac ctxt prems)
-      end ) ctxt)
+      ) ctxt)
   end
 \<close>
 
 lemma F_strong:
   "rel_F R1 id id R4 id x y \<Longrightarrow> rel_F Q1 id id Q4 id x y \<Longrightarrow> rel_F  (inf R1 Q1) id id (inf R4 Q4) id x y"
-  apply (tactic \<open>mk_F_strong_tac (MRBNF_Def.mrbnf_of @{context} @{type_name F} |> the) @{thm F.map_id} @{thm mr_rel_F_def} @{thm F.mr_rel_mono_strong0}
+  by (tactic \<open>mk_F_strong_tac (MRBNF_Def.mrbnf_of @{context} @{type_name F} |> the) @{thm F.map_id} @{thm mr_rel_F_def} @{thm F.mr_rel_mono_strong0}
     @{thm F_rel_map_set2_strong} @{thm F.in_rel} @{context} 
     THEN print_tac @{context} "done"\<close>)
-  done
 
 ML \<open>
 open BNF_Util BNF_Tactics
 
-fun mk_rel_F_exchange_tac F_mr_rel_mono_strong0 F_strong ctxt =
-  HEADGOAL (Subgoal.FOCUS
-    (fn {prems, context = ctxt, ...} => 
-      HEADGOAL (rtac ctxt (F_mr_rel_mono_strong0 
-          OF @{thms supp_id_bound bij_id supp_id_bound supp_id_bound bij_id supp_id_bound})) THEN
-      HEADGOAL (rtac ctxt (F_strong OF prems)) THEN
-      unfold_thms_tac ctxt ([id_apply, eqTrueI OF [refl]] @ @{thms ball_triv inf_apply inf_bool_def}) THEN
-      ALLGOALS (TRY o (rtac ctxt ballI THEN_ALL_NEW rtac ctxt ballI) 
-        THEN_ALL_NEW rtac ctxt impI) THEN
-      HEADGOAL (rtac ctxt TrueI) THEN
-      HEADGOAL (rtac ctxt TrueI) THEN
-      HEADGOAL (etac ctxt conjunct1) THEN
-      HEADGOAL (etac ctxt conjunct2)
-     ) ctxt)
+fun mk_rel_F_exchange_tac mrbnf F_mr_rel_mono_strong0 F_strong ctxt =
+  let
+    val id_prems = MRBNF_Comp_Tactics.mk_id_prems mrbnf;
+  in
+    HEADGOAL (Subgoal.FOCUS
+      (fn {prems, context = ctxt, ...} => 
+        HEADGOAL (EVERY' [
+          rtac ctxt (F_mr_rel_mono_strong0 OF flat (replicate 2 id_prems)),
+          rtac ctxt (F_strong OF prems),
+          K (unfold_thms_tac ctxt ([id_apply, eqTrueI OF [refl]] @ @{thms ball_triv inf_apply inf_bool_def}))
+        ]) THEN
+        ALLGOALS (
+          (rtac ctxt impI THEN' 
+          rtac ctxt TrueI) ORELSE'
+          (rtac ctxt ballI THEN' 
+          rtac ctxt ballI THEN'
+          rtac ctxt impI THEN'
+          eresolve_tac ctxt [conjunct1, conjunct2]))
+       ) ctxt)
+  end
 \<close>
 
 (* Another important consequence: the following "exchange"-property, which could be read: 
 Since the atoms have a fixed position, we can permute the relations: *)
 lemma rel_F_exchange: 
-  fixes x :: "('a1::var,'a2::var,'a3,'a4) F" and x' :: "('a1,'a2,'a3','a4') F"
-  assumes "rel_F id id R2 R3 x x'" and "rel_F id id Q2 Q3 x x'"
-  shows "rel_F id id R2 Q3 x x'" 
+  fixes x :: "('a, 'b :: var, 'c :: var, 'd, 'e :: var, 'f) F" and x' :: "('a', 'b, 'c, 'd', 'e, 'f) F"
+  assumes "rel_F R1 id id R4 id x x'" and "rel_F Q1 id id Q4 id x x'"
+  shows "rel_F R1 id id Q4 id x x'" 
   using assms apply -
-  apply (tactic \<open>mk_rel_F_exchange_tac @{thm F.mr_rel_mono_strong0} @{thm F_strong} @{context} 
-    THEN print_tac @{context} "done" THEN no_tac\<close>)
-  subgoal premises prems
-    apply (rule F.mr_rel_mono_strong0[OF supp_id_bound bij_id supp_id_bound supp_id_bound bij_id supp_id_bound])
-    apply (rule F_strong[OF prems])
-       apply (unfold id_apply eqTrueI[OF refl] ball_triv inf_apply inf_bool_def)
-       apply (intro impI TrueI)
-       apply (intro impI TrueI)
-     apply (intro ballI impI)
-     apply (erule conjunct1)
-    apply (intro ballI impI)
-    apply (erule conjunct2)
-    done
-  done
+  by (tactic \<open>mk_rel_F_exchange_tac (MRBNF_Def.mrbnf_of @{context} @{type_name F} |> the) 
+    @{thm F.mr_rel_mono_strong0} @{thm F_strong} @{context} 
+    THEN print_tac @{context} "done"\<close>)
 
+(* Then notion of two items having the same shape (w.r.t. the 1st position): *)
+(* these definitions are lin_pos dependent *)
+definition sameShape1 :: "('a1,'a2::var,'a3::var,'a4,'a5::var,'a6) F \<Rightarrow> ('a1,'a2,'a3,'a4,'a5,'a6) F \<Rightarrow> bool" where 
+  "sameShape1 x x' \<equiv> \<exists> R. rel_F R id id (=) id x x'"
 
-(* Then notion of two items having the same shape (w.r.t. the 3rd position): *)
-definition sameShape1 :: "('a1::var,'a2::var,'a3,'a4) F \<Rightarrow> ('a1,'a2,'a3,'a4) F \<Rightarrow> bool" where 
-  "sameShape1 x x' \<equiv> \<exists> R. rel_F id id R (=) x x'"
+definition nonrep2 :: "('a1,'a2::var,'a3::var,'a4,'a5::var,'a6) F \<Rightarrow> bool" where 
+  "nonrep2 x \<equiv> \<forall> x'. sameShape1 x x' \<longrightarrow> (\<exists> f. x' = map_F f id id id id x)"
 
-definition nonrep2 :: "('a1::var,'a2::var,'a3,'a4) F \<Rightarrow> bool" where 
-  "nonrep2 x \<equiv> \<forall> x'. sameShape1 x x' \<longrightarrow> (\<exists> f. x' = map_F id id f id x)"
-
-(* this is not used anywhere. A ML tactic is not needed then? *)
-lemma op_eq_triv_sym: "(\<lambda>x. (=) (g x)) = (\<lambda>x z. z = g x)"
-  apply (intro ext)
-  apply (rule eq_commute)
-  done
 
 ML\<open>
 open BNF_Util BNF_Tactics
 
-fun mk_nonrep2_map_F_tac nonrep_def sameShape_def F_map_comp F_mr_rel_map mr_rel_F_def F_rel_compp 
-  F_rel_Grp F_map_id F_in_rel F_rel_map1 F_rel_map2 F_rel_refl_strong ctxt = 
+fun mk_nonrep2_map_F_tac mrbnf nonrep_def sameShape_def F_map_comp F_mr_rel_map mr_rel_F_def F_rel_compp 
+  F_rel_Grp F_map_id F_in_rel F_rel_maps F_rel_refl_strong ctxt = 
   HEADGOAL (Subgoal.FOCUS 
     (fn {prems, context = ctxt, ...} => 
       let
-        val unfold_map_comp = F_map_comp OF ((take 3 prems) @ @{thms supp_id_bound bij_id supp_id_bound});
-        val fold_map_comp = F_map_comp OF (@{thms supp_id_bound bij_id supp_id_bound} @ (take 3 prems)) RS sym;
+        val var_types = var_types_of_mrbnf mrbnf;
+        val nr_lives = length (filter (fn v => v = MRBNF_Def.Live_Var) var_types);
+        val nr_non_lives = length (filter (fn v => not (v = MRBNF_Def.Live_Var)) var_types);
+        val lin_live_pos = fold_index (fn (i, v) => fn b => 
+          if (v = MRBNF_Def.Live_Var andalso i+1 < lin_pos) then b+1 else b) var_types 1;
+        val switch_poses = map_range (fn i => if i < (lin_pos-(lin_live_pos)) then i+1 else i+2) (nr_non_lives);
         val switch = (fn thm1 => (fn thm2 => trans OF [thm1, thm2 RS sym]));
         val o_id = @{thm o_id};
         val id_o = @{thm id_o};
@@ -210,26 +172,30 @@ fun mk_nonrep2_map_F_tac nonrep_def sameShape_def F_map_comp F_mr_rel_map mr_rel
           rtac ctxt allI,
           rtac ctxt impI,
           etac ctxt exE,
-          EqSubst.eqsubst_tac ctxt [0] [unfold_map_comp],
-          EqSubst.eqsubst_tac ctxt [1] [switch o_id id_o],
-          EqSubst.eqsubst_tac ctxt [1, 2, 4] [switch id_o o_id],
-          EqSubst.eqsubst_tac ctxt [0] [fold_map_comp],
-          dtac ctxt (F_mr_rel_map OF ((take 3 prems) @ @{thms supp_id_bound bij_id supp_id_bound}) RS iffD1),
-          EqSubst.eqsubst_asm_tac ctxt [1, 2] [switch id_o o_id],
-          EqSubst.eqsubst_asm_tac ctxt [0] @{thms Grp_UNIV_id},
-          EqSubst.eqsubst_asm_tac ctxt [1] [switch @{thm OO_eq} @{thm eq_OO}],
-          EqSubst.eqsubst_asm_tac ctxt [1] [switch @{thm eq_OO} @{thm OO_eq}],
-          EqSubst.eqsubst_asm_tac ctxt [1, 2] @{thms eq_alt}          
+          EqSubst.eqsubst_tac ctxt [0] [F_map_comp] THEN_ALL_NEW
+            TRY o resolve_tac ctxt (prems @ @{thms supp_id_bound bij_id}),
+          K (unfold_tac ctxt [switch id_o o_id]),
+          EqSubst.eqsubst_tac ctxt [lin_pos] [switch o_id id_o], (*move all id to the right except for lin_pos*)
+          EqSubst.eqsubst_tac ctxt [0] [F_map_comp RS sym] THEN_ALL_NEW
+            TRY o resolve_tac ctxt (prems @ @{thms supp_id_bound bij_id}),
+          dtac ctxt (rotate_prems ~1 (F_mr_rel_map RS iffD1)) THEN_ALL_NEW
+            TRY o resolve_tac ctxt (prems @ @{thms supp_id_bound bij_id}),
+          K (unfold_tac ctxt [switch id_o o_id, @{thm Grp_UNIV_id}]),
+          K (unfold_tac ctxt [switch @{thm OO_eq} @{thm eq_OO}]),  
+          EqSubst.eqsubst_asm_tac ctxt [lin_live_pos] [switch @{thm eq_OO} @{thm OO_eq}], (*move all (=) to the right except for lin_live_pos*)
+          K (unfold_tac ctxt @{thms eq_alt}),   
+          EqSubst.eqsubst_tac ctxt [0] @{thms Grp_UNIV_id}
         ]) THEN
         unfold_thms_tac ctxt [mr_rel_F_def, o_id, F_rel_compp, F_rel_Grp, F_map_id] THEN
         unfold_thms_tac ctxt [eqTrueI OF @{thms subset_UNIV}, @{thm simp_thms(21)}, id_o, @{thm UNIV_def} RS sym] THEN
-        unfold_thms_tac ctxt ((eqTrueI OF [@{thm UNIV_I}]):: @{thms Grp_UNIV_id OO_def Grp_def simp_thms(21)}) THEN
+        unfold_thms_tac ctxt ([eqTrueI OF [@{thm UNIV_I}], id_apply] @ @{thms Grp_UNIV_id OO_def Grp_def simp_thms(21)}) THEN
         HEADGOAL (EVERY' [
-          EqSubst.eqsubst_asm_tac ctxt [1] [id_apply],
           etac ctxt exE,
           etac ctxt conjE,
-          dtac ctxt (F_in_rel OF (take 3 prems) RS iffD1),
-          Method.insert_tac ctxt [unfold_thms ctxt [nonrep_def, sameShape_def, mr_rel_F_def, F_map_id] (nth prems 3)],
+          dtac ctxt (rotate_prems ~1 (F_in_rel RS iffD1)) THEN_ALL_NEW
+            TRY o resolve_tac ctxt prems,
+          Method.insert_tac ctxt [unfold_thms ctxt [nonrep_def, sameShape_def, mr_rel_F_def, F_map_id] 
+            (nth prems (length prems -1))],
           etac ctxt exE,
           etac ctxt conjE,
           etac ctxt CollectE,
@@ -243,20 +209,21 @@ fun mk_nonrep2_map_F_tac nonrep_def sameShape_def F_map_comp F_mr_rel_map mr_rel
               Method.insert_tac ctxt [nth subprems 0],
               etac ctxt allE,
               etac ctxt impE,
-              rtac ctxt (infer_instantiate' ctxt [NONE, SOME (snd (nth params 1))] exI),
-              EqSubst.eqsubst_tac ctxt [1] [F_rel_map1],
-              EqSubst.eqsubst_tac ctxt [1] [F_rel_map2],
-              rtac ctxt F_rel_refl_strong,
-              dtac ctxt (subsetD OF [nth subprems 1] RS @{thm Collect_case_prodD}),
-              assume_tac ctxt,
-              dtac ctxt (subsetD OF [nth subprems 2] RS @{thm Collect_case_prodD}),
-              rtac ctxt sym,
-              assume_tac ctxt,
+              rtac ctxt (infer_instantiate' ctxt [NONE, SOME (snd (nth params 1))] exI)
+            ]) THEN
+            REPEAT_DETERM_N nr_lives (HEADGOAL (EqSubst.eqsubst_tac ctxt [1] F_rel_maps)) THEN
+            HEADGOAL (EVERY' [
+              rtac ctxt F_rel_refl_strong THEN_ALL_NEW
+                (dresolve_tac ctxt (map (fn p => subsetD OF [p] RS @{thm Collect_case_prodD}) (drop 1 subprems)) THEN'
+                  (assume_tac ctxt ORELSE' 
+                  (rtac ctxt sym THEN' assume_tac ctxt))),
 
               etac ctxt exE,
-              EqSubst.eqsubst_tac ctxt [0] [unfold_map_comp],
-              EqSubst.eqsubst_tac ctxt [1, 2] [switch id_o o_id],
-              EqSubst.eqsubst_tac ctxt [0] [fold_map_comp],
+              EqSubst.eqsubst_tac ctxt [0] [F_map_comp] THEN_ALL_NEW
+                TRY o resolve_tac ctxt (prems @ @{thms supp_id_bound bij_id}),
+              EqSubst.eqsubst_tac ctxt switch_poses [switch id_o o_id],
+              EqSubst.eqsubst_tac ctxt [0] [F_map_comp RS sym] THEN_ALL_NEW
+                TRY o resolve_tac ctxt (prems @ @{thms supp_id_bound bij_id}),
               rtac ctxt exI,
               dtac ctxt arg_cong,
               assume_tac ctxt
@@ -267,80 +234,32 @@ fun mk_nonrep2_map_F_tac nonrep_def sameShape_def F_map_comp F_mr_rel_map mr_rel
 \<close>
 
 lemma nonrep2_map_F:
-  fixes x :: "('a1::var,'a2::var,'a3,'a4) F"
-    and v :: "'a1 \<Rightarrow> 'a1" and u :: "'a2\<Rightarrow>'a2" and g :: "'a4 \<Rightarrow> 'b4"
-  assumes v: "|supp v| <o |UNIV :: 'a1 set|"  and u: "bij u" "|supp u| <o |UNIV :: 'a2 set|" 
+  fixes x :: "('a1,'a2::var,'a3::var,'a4,'a5::var,'a6) F"
+    and u2 :: "'a2 \<Rightarrow> 'a2" and v3 :: "'a3\<Rightarrow>'a3" and u5 :: "'a5\<Rightarrow>'a5" and g :: "'a4 \<Rightarrow> 'b4"
+  assumes "bij u2" "|supp u2| <o |UNIV :: 'a2 set|" 
+    and "|supp v3| <o |UNIV :: 'a3 set|" 
+    and "bij u5" "|supp u5| <o |UNIV :: 'a5 set|" 
   assumes "nonrep2 x"
-  shows "nonrep2 (map_F v u id g x)"
+  shows "nonrep2 (map_F id u2 v3 g u5 x)"
   using assms apply -
-  apply (tactic \<open>mk_nonrep2_map_F_tac @{thm nonrep2_def} @{thm sameShape1_def} @{thm F.map_comp} 
-    @{thm F.mr_rel_map(1)} @{thm mr_rel_F_def} @{thm F.rel_compp} @{thm F.rel_Grp} @{thm F.map_id}
-    @{thm F.in_rel} @{thm F.rel_map(1)} @{thm F.rel_map(2)} @{thm F.rel_refl_strong}
-    @{context}
-    THEN print_tac @{context} "done" THEN no_tac\<close>)
-  subgoal premises prems
-    apply (unfold nonrep2_def sameShape1_def)
-    apply (rule allI)
-    apply (rule impI)
-    apply (elim exE)
-    apply (subst F.map_comp[OF prems(1,2,3) supp_id_bound bij_id supp_id_bound])
-    apply (subst (1) trans[OF o_id id_o[symmetric]])
-    apply (subst (1 2 4) trans[OF id_o o_id[symmetric]])
-    apply (subst F.map_comp[OF supp_id_bound bij_id supp_id_bound prems(1,2,3), symmetric])
-    apply (drule iffD1[OF F.mr_rel_map(1)[OF prems(1,2,3) supp_id_bound bij_id supp_id_bound]])
-    apply (subst (asm) (1 2) trans[OF id_o o_id[symmetric]])
-    apply (subst (asm) Grp_UNIV_id)
-    apply (subst (asm) trans[OF OO_eq eq_OO[symmetric]])
-    apply (subst (asm) trans[OF eq_OO OO_eq [symmetric]])
-    apply (subst (asm) (1 2) eq_alt)
-    apply (unfold mr_rel_F_def o_id F.rel_compp F.rel_Grp F.map_id)
-    apply (unfold eqTrueI[OF subset_UNIV] simp_thms(21) UNIV_def[symmetric] id_o)
-    apply (unfold Grp_UNIV_id OO_def Grp_def eqTrueI[OF UNIV_I] simp_thms(21))
-    apply (subst (asm) id_apply)
-    apply (erule exE)
-    apply (erule conjE)
-    apply (drule iffD1[OF F.in_rel[OF prems(1,2,3)]])
-    apply (insert prems(4)[unfolded nonrep2_def sameShape1_def mr_rel_F_def F.map_id])
-    apply (erule exE)
-    apply (erule conjE)
-    apply (erule CollectE)
-    apply (erule conjE)
-    apply (erule conjE)
-    apply (hypsubst_thin)
-    subgoal premises subprems for x' R y z
-      apply (insert subprems(1))
-      apply (erule allE)
-      apply (erule impE)
-(* this instantiation of R is not really necessary, but it feels better to have it concretely *)
-       apply (rule exI[of _ R])
-       apply (subst F.rel_map(1))
-       apply (subst F.rel_map(2))
-       apply (rule F.rel_refl_strong)
-        apply (drule subsetD[OF subprems(2), THEN Collect_case_prodD])
-        apply (assumption)
-       apply (drule subsetD[OF subprems(3), THEN Collect_case_prodD])
-       apply (rule sym)
-       apply (assumption)
-
-      apply (elim exE)
-      apply (subst F.map_comp[OF prems(1,2,3) supp_id_bound bij_id supp_id_bound])
-      apply (subst (1 2) trans[OF id_o o_id[symmetric]])
-      apply (subst F.map_comp[OF supp_id_bound bij_id supp_id_bound prems(1,2,3), symmetric])
-      apply (rule exI)
-      apply (drule arg_cong)
-      apply (assumption)
-      done
-    done
-  done
+  by (tactic \<open>mk_nonrep2_map_F_tac (MRBNF_Def.mrbnf_of @{context} @{type_name F} |> the) @{thm nonrep2_def} 
+    @{thm sameShape1_def} @{thm F.map_comp}  @{thm F.mr_rel_map(1)} @{thm mr_rel_F_def} @{thm F.rel_compp} 
+    @{thm F.rel_Grp} @{thm F.map_id} @{thm F.in_rel} @{thms F.rel_map} @{thm F.rel_refl_strong}
+    @{context} THEN print_tac @{context} "done"\<close>)
 
 ML\<open>
 open BNF_Util BNF_Tactics
 
-fun mk_nonrep2_map_F_rev_tac nonrep_def sameShape_def F_mr_rel_map1 F_mr_rel_map2 F_mr_rel_map3 F_map_comp F_rel_eq 
+fun mk_nonrep2_map_F_rev_tac mrbnf nonrep_def sameShape_def F_mr_rel_map1 F_mr_rel_map2 F_mr_rel_map3 F_map_comp F_rel_eq 
   F_mr_rel_id rel_F_exchange F_mr_rel_flip F_mr_rel_mono_strong0 F_mr_rel_Grp ctxt = 
   HEADGOAL (Subgoal.FOCUS 
     (fn {prems, context = ctxt, ...} => 
       let
+        val var_types = var_types_of_mrbnf mrbnf;
+        val nr_lives = length (filter (fn v => v = MRBNF_Def.Live_Var) var_types);
+        val nr_non_lives = length (filter (fn v => not (v = MRBNF_Def.Live_Var)) var_types);
+        val lin_live_pos = fold_index (fn (i, v) => fn b => 
+          if (v = MRBNF_Def.Live_Var andalso i+1 < lin_pos) then b+1 else b) var_types 1;
         val switch = (fn thm1 => (fn thm2 => trans OF [thm1, thm2 RS sym]));
       in
         unfold_thms_tac ctxt [nonrep_def, sameShape_def] THEN
@@ -351,14 +270,14 @@ fun mk_nonrep2_map_F_rev_tac nonrep_def sameShape_def F_mr_rel_map1 F_mr_rel_map
           forward_tac ctxt [rotate_prems ~1 F_mr_rel_map2] THEN_ALL_NEW
             TRY o resolve_tac ctxt (prems @ @{thms supp_id_bound bij_id}),
           rotate_tac 1,
-          EqSubst.eqsubst_asm_tac ctxt [2] [switch @{thm o_id} @{thm id_o}],
-          EqSubst.eqsubst_asm_tac ctxt [0] @{thms Grp_UNIV_id},
-          EqSubst.eqsubst_asm_tac ctxt [0] [switch @{thm eq_OO} @{thm OO_eq}],
-          EqSubst.eqsubst_asm_tac ctxt [0] [switch @{thm OO_eq} @{thm eq_OO}],
-          EqSubst.eqsubst_asm_tac ctxt [0] @{thms eq_alt},
+          EqSubst.eqsubst_asm_tac ctxt (map_range (fn i => i+1) nr_non_lives) [switch @{thm o_id} @{thm id_o}],
+          EqSubst.eqsubst_asm_tac ctxt [lin_live_pos] @{thms Grp_UNIV_id},
+          K (unfold_tac ctxt [switch @{thm eq_OO} @{thm OO_eq}]),
+          EqSubst.eqsubst_asm_tac ctxt [lin_live_pos] [switch @{thm OO_eq} @{thm eq_OO}], (*move all (=) to the right and then lin_live_pos back*)
+          EqSubst.eqsubst_asm_tac ctxt [lin_live_pos] @{thms eq_alt},
           EqSubst.eqsubst_asm_tac ctxt [0] [F_mr_rel_map1 RS sym] THEN_ALL_NEW
             TRY o resolve_tac ctxt (prems @ @{thms supp_id_bound bij_id}),
-          Method.insert_tac ctxt [unfold_thms ctxt [nonrep_def, sameShape_def] (nth prems 2)],
+          Method.insert_tac ctxt [unfold_thms ctxt [nonrep_def, sameShape_def] (nth prems (length prems - 1))],
           etac ctxt allE,
           etac ctxt impE,
           rtac ctxt exI,
@@ -367,39 +286,50 @@ fun mk_nonrep2_map_F_rev_tac nonrep_def sameShape_def F_mr_rel_map1 F_mr_rel_map
           etac ctxt exE,
           EqSubst.eqsubst_asm_tac ctxt [0] [F_map_comp] THEN_ALL_NEW
             TRY o resolve_tac ctxt (prems @ @{thms supp_id_bound bij_id}),
-          K (unfold_thms_tac ctxt @{thms id_o o_id}),
+          K (unfold_tac ctxt @{thms id_o o_id}),
           EqSubst.eqsubst_asm_tac ctxt [1] [F_rel_eq RS sym],
           EqSubst.eqsubst_asm_tac ctxt [1] [F_mr_rel_id],
           dtac ctxt (rotate_prems ~1 (iffD1 OF [F_mr_rel_map1])) THEN_ALL_NEW
             TRY o resolve_tac ctxt (prems @ @{thms supp_id_bound bij_id}),
-          K (unfold_thms_tac ctxt @{thms id_o OO_eq}),
+          K (unfold_tac ctxt @{thms id_o OO_eq}),
           dtac ctxt (rotate_prems 1 rel_F_exchange),
-          rtac ctxt (unfold_thms ctxt @{thms inv_id} (F_mr_rel_flip OF @{thms bij_id supp_id_bound bij_id supp_id_bound}) RS iffD1),
+          rtac ctxt (F_mr_rel_flip RS iffD1) THEN_ALL_NEW
+            TRY o resolve_tac ctxt @{thms supp_id_bound bij_id},
+          K (unfold_tac ctxt @{thms inv_id}),
           EqSubst.eqsubst_asm_tac ctxt [0] [F_mr_rel_map3] THEN_ALL_NEW
             TRY o resolve_tac ctxt (prems @ @{thms supp_id_bound bij_id}),
-          EqSubst.eqsubst_asm_tac ctxt [1, 2, 3, 4] @{thms Grp_def},
-          EqSubst.eqsubst_asm_tac ctxt [0] [@{thm inv_o_simp1} OF @{thms bij_id}],
-          EqSubst.eqsubst_asm_tac ctxt [0] [@{thm inv_o_simp1} OF [(nth prems 0)]],
-          EqSubst.eqsubst_asm_tac ctxt [0] @{thms id_apply},
-          K (unfold_thms_tac ctxt [eqTrueI OF @{thms UNIV_I}, @{thm simp_thms(21)}]),
-          EqSubst.eqsubst_asm_tac ctxt [0] @{thms eq_commute},
-          EqSubst.eqsubst_asm_tac ctxt [0] @{thms eq_OO},
-          K (unfold_thms_tac ctxt @{thms conversep_def}),
-          etac ctxt (rotate_prems 6 F_mr_rel_mono_strong0) THEN_ALL_NEW
-            TRY o resolve_tac ctxt (ballI:: @{thms supp_id_bound bij_id}) THEN_ALL_NEW
-            TRY o resolve_tac ctxt [refl, ballI] THEN_ALL_NEW
-            TRY o rtac ctxt impI,
-          rotate_tac 2,
-          EqSubst.eqsubst_asm_tac ctxt [0] @{thms eq_commute},
-          assume_tac ctxt,
-          K (unfold_thms_tac ctxt @{thms OO_def}),
-          assume_tac ctxt,
-          etac ctxt thin_rl,
-          EqSubst.eqsubst_asm_tac ctxt [0] [@{thm Grp_UNIV_def} RS sym],
-          rtac ctxt exI,
-          EqSubst.eqsubst_asm_tac ctxt [0] @{thms eq_alt}
+          EqSubst.eqsubst_asm_tac ctxt (map_range (fn i => i+1) (2 * nr_lives)) @{thms Grp_def},
+          EqSubst.eqsubst_asm_tac ctxt (map_range (fn i => i+1) (nr_non_lives)) @{thms inv_o_simp1} THEN_ALL_NEW
+            TRY o resolve_tac ctxt (@{thm bij_id}::prems),
+          K (unfold_thms_tac ctxt ((eqTrueI OF @{thms UNIV_I}):: @{thms id_apply simp_thms(21)})),
+          EqSubst.eqsubst_asm_tac ctxt [lin_live_pos] @{thms eq_commute},
+          K (unfold_thms_tac ctxt @{thms eq_OO conversep_def}),
+          etac ctxt (rotate_prems (~1 - (length var_types)) F_mr_rel_mono_strong0) THEN_ALL_NEW
+            TRY o resolve_tac ctxt @{thms supp_id_bound bij_id}
         ]) THEN
-        unfold_thms_tac ctxt [F_mr_rel_Grp OF @{thms supp_id_bound bij_id supp_id_bound}] THEN
+        REPEAT_DETERM_N (length var_types) (
+          (HEADGOAL (
+            (* for bound and free *)
+            rtac ctxt ballI THEN'
+            rtac ctxt refl)) 
+          ORELSE 
+          (HEADGOAL (
+            (* for lives*)
+            rtac ctxt ballI THEN'
+            rtac ctxt ballI THEN'
+            rtac ctxt impI THEN'
+            rotate_tac 2 THEN'
+            EqSubst.eqsubst_asm_tac ctxt [0] @{thms eq_commute} THEN'
+            assume_tac ctxt))
+        ) THEN
+        HEADGOAL (EVERY' [
+          etac ctxt thin_rl,
+          EqSubst.eqsubst_asm_tac ctxt [lin_live_pos] [@{thm Grp_UNIV_def} RS sym],
+          rtac ctxt exI,
+          EqSubst.eqsubst_asm_tac ctxt (map_range (fn i => i+1) (nr_lives -1)) @{thms eq_alt},
+          EqSubst.eqsubst_asm_tac ctxt [0] [F_mr_rel_Grp] THEN_ALL_NEW
+            TRY o resolve_tac ctxt @{thms supp_id_bound bij_id}
+        ]) THEN
         unfold_thms_tac ctxt ([eqTrueI OF @{thms subset_UNIV}, eqTrueI OF @{thms UNIV_I}, @{thm UNIV_def} RS sym] @ 
           @{thms simp_thms(21) Grp_def}) THEN
         HEADGOAL (assume_tac ctxt)
@@ -409,183 +339,129 @@ fun mk_nonrep2_map_F_rev_tac nonrep_def sameShape_def F_mr_rel_map1 F_mr_rel_map
 
 (* Here we need pullback preservation: *)
 lemma nonrep2_map_F_rev:
-  fixes x :: "('a1::var,'a2::var,'a3,'a4) F" and u :: "'a2\<Rightarrow>'a2" and g :: "'a4 \<Rightarrow> 'b4"
-  assumes u: "bij u" "|supp u| <o |UNIV :: 'a2 set|" 
-  assumes "nonrep2 (map_F id u id g x)"
+  fixes x :: "('a1,'a2::var,'a3::var,'a4,'a5::var,'a6) F" and u2 :: "'a2\<Rightarrow>'a2" and u5 :: "'a5\<Rightarrow>'a5"  and g :: "'a4 \<Rightarrow> 'a4'"
+  assumes "bij u2" "|supp u2| <o |UNIV :: 'a2 set|" 
+    and "bij u5" "|supp u5| <o |UNIV :: 'a5 set|" 
+  assumes "nonrep2 (map_F id u2 id g u5 x)"
   shows "nonrep2 x"
   using assms apply -
-  apply (tactic \<open>mk_nonrep2_map_F_rev_tac @{thm nonrep2_def} @{thm sameShape1_def} @{thm F.mr_rel_map(1)}
+  by (tactic \<open>mk_nonrep2_map_F_rev_tac (MRBNF_Def.mrbnf_of @{context} @{type_name F} |> the) @{thm nonrep2_def} @{thm sameShape1_def} @{thm F.mr_rel_map(1)}
     @{thm F.mr_rel_map(2)} @{thm F.mr_rel_map(3)} @{thm F.map_comp} @{thm F.rel_eq} @{thm F.mr_rel_id} @{thm rel_F_exchange} 
     @{thm F.mr_rel_flip} @{thm F.mr_rel_mono_strong0} @{thm F.mr_rel_Grp} @{context} 
-    THEN print_tac @{context} "done" THEN no_tac\<close>)
-
-  subgoal premises prems
-    thm F.mr_rel_map(2)[OF supp_id_bound bij_id supp_id_bound supp_id_bound, rotated 2]
-    apply (unfold nonrep2_def sameShape1_def)
-    apply (rule allI)
-    apply (rule impI)
-    apply (erule exE)
-    apply (frule F.mr_rel_map(2)[rotated -1]; (rule prems supp_id_bound bij_id)?)
-    apply (rotate_tac)
-    apply (subst (asm) (2) trans[OF o_id id_o[symmetric]])
-    apply (subst (asm) Grp_UNIV_id)
-    apply (subst (asm) trans[OF eq_OO OO_eq[symmetric]])
-    apply (subst (asm) trans[OF OO_eq eq_OO[symmetric]])
-    apply (subst (asm) eq_alt)
-    apply (subst (asm) F.mr_rel_map(1)[symmetric]; (rule prems supp_id_bound bij_id)?)
-    apply (insert prems(3)[unfolded nonrep2_def sameShape1_def])
-    apply (elim allE impE)
-     apply (rule exI)
-     apply (assumption)
-
-    apply (erule thin_rl)
-    apply (erule exE)
-    apply (subst (asm) F.map_comp; (rule prems supp_id_bound bij_id)?)
-    apply (unfold o_id id_o)
-    apply (subst (asm) (1) F.rel_eq[symmetric])
-    apply (unfold F.mr_rel_id)
-    apply (drule iffD1[OF F.mr_rel_map(1), rotated -1]; (rule prems supp_id_bound bij_id)?)
-    apply (unfold id_o OO_eq)
-
-    apply (drule rel_F_exchange[rotated])
-     apply (rule iffD1[OF F.mr_rel_flip[OF bij_id supp_id_bound bij_id supp_id_bound, unfolded inv_id]])
-    apply (subst (asm) F.mr_rel_map(3); (rule prems supp_id_bound bij_id)?)
-    apply (subst (asm) (1 2 3 4) Grp_def)
-     apply (subst (asm) inv_o_simp1[OF bij_id])
-     apply (subst (asm) inv_o_simp1[OF u(1)])
-     apply (subst (asm) id_apply)
-     apply (unfold eqTrueI[OF UNIV_I] simp_thms(21))
-     apply (subst (asm) eq_commute)
-     apply (subst (asm) eq_OO)
-     apply (unfold conversep_def)
-     apply (elim F.mr_rel_mono_strong0[rotated 6]; (rule supp_id_bound bij_id)?)
-        apply (rule ballI; rule refl)
-       apply (rule ballI; rule refl)
-      apply (intro ballI impI)
-      apply (rotate_tac 2)
-      apply (subst (asm) eq_commute)
-      apply (assumption)
-     apply (intro ballI impI)
-     apply (unfold OO_def)
-     apply (assumption)
-
-    apply (erule thin_rl)
-    apply (subst (asm) Grp_UNIV_def[symmetric])
-    apply (rule exI)
-    apply (subst (asm) eq_alt)
-    apply (unfold F.mr_rel_Grp[OF supp_id_bound bij_id supp_id_bound])
-    apply (unfold eqTrueI[OF subset_UNIV] eqTrueI[OF UNIV_I] UNIV_def[THEN sym] simp_thms(21) Grp_def)
-    apply (assumption)
-    done
-  done
+    THEN print_tac @{context} "done"\<close>)
 
 
-lemma nonrep2_mapF_bij: (* TODO *)
-  fixes x :: "('a1::var,'a2::var,'a3,'a4) F" and g::"'a3\<Rightarrow>'a3"
+ML\<open>
+open BNF_Util BNF_Tactics
+fun mk_nonrep2_map_bij_tac mrbnf nonrep_def sameShape_def F_mr_rel_map1 F_mr_rel_map3 F_map_id F_map_comp ctxt = 
+  HEADGOAL (Subgoal.FOCUS 
+    (fn {prems, context = ctxt, ...} => 
+      let
+        val id_prems = MRBNF_Comp_Tactics.mk_id_prems mrbnf;
+        val id_prems_v = MRBNF_Comp_Tactics.mk_prems mrbnf @{thms bij_id supp_id_bound} @{thms bij_id supp_id_bound}
+        val var_types = var_types_of_mrbnf mrbnf;
+        val nr_lives = length (filter (fn v => v = MRBNF_Def.Live_Var) var_types);
+        val lin_live_pos = fold_index (fn (i, v) => fn b => 
+          if (v = MRBNF_Def.Live_Var andalso i+1 < lin_pos) then b+1 else b) var_types 1;
+        val o_id_poses = map_range (fn i => if i < lin_pos-1 then i*2 + 7 else (i+1)*2 + 7) (length var_types-1) |> filter (fn n => n >= 0);
+      in
+        unfold_tac ctxt [nonrep_def, sameShape_def] THEN
+        HEADGOAL (EVERY' [
+          rtac ctxt allI,
+          rtac ctxt impI,
+          etac ctxt exE,
+          dtac ctxt (rotate_prems ~1 (F_mr_rel_map1 RS iffD1)) THEN_ALL_NEW
+            TRY o resolve_tac ctxt @{thms bij_id supp_id_bound},
+          K (unfold_tac ctxt @{thms o_id Grp_UNIV_id}),
+          EqSubst.eqsubst_asm_tac ctxt [lin_live_pos*3 - 1] [@{thm OO_eq} RS sym],
+          EqSubst.eqsubst_asm_tac ctxt (map_range (fn i => i+1) (nr_lives*2 -1)) [@{thm conversep_eq} RS sym],
+          EqSubst.eqsubst_asm_tac ctxt (map_range (fn i => i+1) (nr_lives*2 -1)) @{thms eq_alt},
+          EqSubst.eqsubst_asm_tac ctxt [1] [@{thm inv_o_simp2} OF [(nth prems 0)] RS sym],
+          K (unfold_tac ctxt @{thms Grp_o converse_relcompp}),
+          EqSubst.eqsubst_asm_tac ctxt [1] [@{thm relcompp_assoc} RS sym],
+          dtac ctxt ((unfold_thms ctxt @{thms inv_id o_id} (F_mr_rel_map3 OF 
+            (id_prems @ id_prems_v) RS sym)) RS iffD1),
+          K (unfold_tac ctxt @{thms Grp_UNIV_id conversep_eq}),
+          dtac ctxt (Object_Logic.rulify ctxt (unfold_thms ctxt [nonrep_def, sameShape_def] (nth prems 1)) OF [exI]),
+          etac ctxt exE
+        ]) THEN
+        HEADGOAL (Subgoal.FOCUS 
+          (fn {prems = subprems, context = ctxt, ...} => 
+            HEADGOAL (EVERY' [
+              EqSubst.eqsubst_tac ctxt [0] [F_map_id RS sym],
+              EqSubst.eqsubst_tac ctxt o_id_poses [@{thm o_id} RS sym],
+              EqSubst.eqsubst_tac ctxt [1] [@{thm inv_o_simp2} OF [(nth prems 0)] RS sym],
+              K (unfold_tac ctxt [F_map_comp OF flat (replicate 2 id_prems) RS sym]),
+              EqSubst.eqsubst_tac ctxt [1] subprems,
+              EqSubst.eqsubst_tac ctxt [2*lin_pos + 6 + 2*(length var_types)] [@{thm o_id} RS sym],
+              EqSubst.eqsubst_tac ctxt [1] [@{thm inv_o_simp1} OF [(nth prems 0)] RS sym],
+              K (unfold_tac ctxt [F_map_comp OF flat (replicate 2 id_prems)]),
+              EqSubst.eqsubst_tac ctxt [1, 2] @{thms o_assoc},
+              rtac ctxt exI,
+              rtac ctxt refl
+            ])
+          ) ctxt)
+      end)
+  ctxt)
+\<close>
+
+lemma nonrep2_mapF_bij:
+  fixes x :: "('a1,'a2::var,'a3::var,'a4,'a5::var,'a6) F" and g::"'a1\<Rightarrow>'a1"
   assumes g: "bij g" and x: "nonrep2 x"
-  shows "nonrep2 (map_F id id g id x)" (is "nonrep2 ?x'")
+  shows "nonrep2 (map_F g id id id id x)" (is "nonrep2 ?x'")
   using assms apply -
-  subgoal premises prems
-    apply (unfold nonrep2_def sameShape1_def)
-    apply (rule allI)
-    apply (rule impI)
-    apply (erule exE)
-    subgoal premises subprems for y' R'
-      apply (insert subprems)
-      apply (drule iffD1[OF F.mr_rel_map(1)[OF supp_id_bound bij_id supp_id_bound supp_id_bound bij_id supp_id_bound]])
-      apply (unfold o_id)
-  apply (subst (asm) Grp_UNIV_id)
-  apply (subst (asm) (2) conversep_eq[symmetric])
-  apply (subst (asm) (2) Grp_UNIV_id[symmetric])
-      thm 
-        subprems[THEN iffD1[OF F.mr_rel_map(1)[OF supp_id_bound bij_id supp_id_bound supp_id_bound bij_id supp_id_bound], unfolded o_id]]
-        F.mr_rel_map(3)[OF supp_id_bound bij_id supp_id_bound bij_id supp_id_bound bij_id supp_id_bound, symmetric, 
-            unfolded inv_id o_id]
-        F.mr_rel_map(3)[OF supp_id_bound bij_id supp_id_bound bij_id supp_id_bound bij_id supp_id_bound,
-              of "Grp g OO R' OO conversep (Grp g)" _ _ "inv g" id, symmetric,
-              unfolded inv_id o_id, of "(=)" x y']
-        F.mr_rel_map(3)[OF supp_id_bound bij_id supp_id_bound bij_id supp_id_bound bij_id supp_id_bound,
-              of "Grp g OO R' OO conversep (Grp g)" _ _ "inv g" id, symmetric,
-              unfolded Grp_UNIV_id conversep_eq OO_eq inv_id comp_id relcompp_assoc converse_relcompp[symmetric] Grp_o[symmetric]
-              inv_o_simp2[OF g], of "(=)" x y']
+  by (tactic \<open>mk_nonrep2_map_bij_tac (MRBNF_Def.mrbnf_of @{context} @{type_name F} |> the) @{thm nonrep2_def}
+    @{thm sameShape1_def} @{thm F.mr_rel_map(1)} @{thm F.mr_rel_map(3)} @{thm F.map_id} @{thm F.map_comp} @{context}
+    THEN print_tac @{context} "done"\<close>)
 
-      thm Grp_UNIV_id conversep_eq OO_eq inv_id comp_id relcompp_assoc converse_relcompp[symmetric] Grp_o[symmetric]
-              inv_o_simp2[OF g]
-      apply (drule iffD1[OF F.mr_rel_map(3)[OF supp_id_bound bij_id supp_id_bound bij_id supp_id_bound bij_id supp_id_bound,
-              of "Grp g OO R' OO conversep (Grp g)" _ _ "inv g" id, symmetric,
-              unfolded Grp_UNIV_id conversep_eq OO_eq inv_id comp_id relcompp_assoc converse_relcompp[symmetric] Grp_o[symmetric]
-              inv_o_simp2[OF g]]])
-      thm x[unfolded nonrep2_def sameShape1_def, rule_format, OF exI]
-      apply (drule x[unfolded nonrep2_def sameShape1_def, rule_format, OF exI])
-      apply (erule exE)
-      subgoal premises subprems2 for f
-        apply (subst F.map_id[symmetric])
-        apply (subst (7 9 13) o_id[symmetric])
-        apply (subst inv_o_simp2[OF g, symmetric])
-        apply (fold F.map_comp[OF supp_id_bound bij_id supp_id_bound supp_id_bound bij_id supp_id_bound])
-        apply (subst subprems2)
-        apply (subst (20) o_id[symmetric])
-        apply (subst inv_o_simp1[OF g, symmetric])
-        apply (unfold F.map_comp[OF supp_id_bound bij_id supp_id_bound supp_id_bound bij_id supp_id_bound])
-        apply (subst (1 2) o_assoc)
-        apply (rule exI)
-        apply (rule refl)
-        done
-      done
-    done
-  done
-  sorry
-
-lemma "(Grp id OO (=)) = ((=) OO (Grp id)\<inverse>\<inverse>)"
-  apply (rule refl)
 
 ML \<open>
 open BNF_Util BNF_Tactics
 
-fun mk_nonrep2_mapF_bij_2_tac nonrep2_mapF_bij nonrep2_map_F F_map_comp ctxt =
+fun mk_nonrep2_mapF_bij_2_tac mrbnf nonrep2_mapF_bij nonrep2_map_F F_map_comp ctxt =
   HEADGOAL (Subgoal.FOCUS
     (fn {prems, context = ctxt, ...} => 
-    let val nr_prems = length prems in
-      HEADGOAL (rtac ctxt (unfold_thms ctxt ((F_map_comp OF ((take (nr_prems-2) prems) @ @{thms supp_id_bound bij_id supp_id_bound})) :: @{thms id_o o_id}) 
+    let val nr_prems = length prems;
+        val id_prems = MRBNF_Comp_Tactics.mk_id_prems mrbnf;
+    in
+      HEADGOAL (rtac ctxt (unfold_thms ctxt ((F_map_comp OF ((take (nr_prems-2) prems) @ id_prems)) :: @{thms id_o o_id}) 
         (nonrep2_mapF_bij OF [nth prems (nr_prems-2), nonrep2_map_F OF (nth_drop (nr_prems-2) prems)])
       ))
      end) ctxt)
 \<close>
 
 lemma nonrep2_mapF_bij_2:
-  fixes x :: "('a1::var,'a2::var,'a3,'a4) F"
-    and v :: "'a1 \<Rightarrow> 'a1" and u :: "'a2\<Rightarrow>'a2" and g::"'a3\<Rightarrow>'a3" and f::"'a4\<Rightarrow>'a4'"
-  assumes v: "|supp v| <o |UNIV :: 'a1 set|" and u: "bij u" "|supp u| <o |UNIV :: 'a2 set|"
+  fixes x :: "('a1,'a2::var,'a3::var,'a4,'a5::var,'a6) F"
+    and g :: "'a1 \<Rightarrow> 'a1" and u2 :: "'a2\<Rightarrow>'a2" and v3::"'a3\<Rightarrow>'a3" and f::"'a4\<Rightarrow>'a4'" and u5::"'a5\<Rightarrow>'a5"
+  assumes u2: "bij u2" "|supp u2| <o |UNIV :: 'a2 set|" and v3: "|supp v3| <o |UNIV :: 'a3 set|"
+    and u5: "bij u5" "|supp u5| <o |UNIV :: 'a5 set|"
     and g: "bij g" and x: "nonrep2 x"
-  shows "nonrep2 (map_F v u g f x)" 
+  shows "nonrep2 (map_F g u2 v3 f u5 x)" 
   using assms apply -
-  apply (tactic \<open>mk_nonrep2_mapF_bij_2_tac @{thm nonrep2_mapF_bij} @{thm nonrep2_map_F} @{thm F.map_comp} @{context} 
-    THEN print_tac @{context} "done" THEN no_tac\<close>)
-  subgoal premises prems
-    apply (rule nonrep2_mapF_bij[OF prems(4) nonrep2_map_F[OF prems(1,2,3,5)], 
-          unfolded F.map_comp[OF prems(1,2,3) supp_id_bound bij_id supp_id_bound] id_o o_id])
-    done
-  done
+  by (tactic \<open>mk_nonrep2_mapF_bij_2_tac (MRBNF_Def.mrbnf_of @{context} @{type_name F} |> the) 
+    @{thm nonrep2_mapF_bij} @{thm nonrep2_map_F} @{thm F.map_comp} @{context} 
+    THEN print_tac @{context} "done"\<close>)
 
 
-typedef ('a1::var,'a2::var,'a3::var,'a4) F' = "{x :: ('a1,'a2,'a3,'a4) F. nonrep2 x}"
+typedef ('a1,'a2::var,'a3::var,'a4,'a5::var,'a6) F' = "{x :: ('a1,'a2,'a3,'a4,'a5,'a6) F. nonrep2 x}"
   apply (unfold mem_Collect_eq nonrep2_def sameShape1_def mr_rel_F_def F.map_id id_apply)
   apply (unfold id_def[symmetric])
   by (rule ex_nonrep)
 
-definition set1_F' :: "('a1::var,'a2::var,'a3::var,'a4) F' \<Rightarrow> 'a1 set" where "set1_F' = set1_F o Rep_F'"
-definition set2_F' :: "('a1::var,'a2::var,'a3::var,'a4) F' \<Rightarrow> 'a2 set" where "set2_F' = set2_F o Rep_F'"
-definition set3_F' :: "('a1::var,'a2::var,'a3::var,'a4) F' \<Rightarrow> 'a3 set" where "set3_F' = set3_F o Rep_F'"
-definition set4_F' :: "('a1::var,'a2::var,'a3::var,'a4) F' \<Rightarrow> 'a4 set" where "set4_F' = set4_F o Rep_F'"
+definition set1_F' :: "('a1,'a2::var,'a3::var,'a4,'a5::var,'a6) F' \<Rightarrow> 'a1 set" where "set1_F' = set1_F o Rep_F'"
+definition set2_F' :: "('a1,'a2::var,'a3::var,'a4,'a5::var,'a6) F' \<Rightarrow> 'a2 set" where "set2_F' = set2_F o Rep_F'"
+definition set3_F' :: "('a1,'a2::var,'a3::var,'a4,'a5::var,'a6) F' \<Rightarrow> 'a3 set" where "set3_F' = set3_F o Rep_F'"
+definition set4_F' :: "('a1,'a2::var,'a3::var,'a4,'a5::var,'a6) F' \<Rightarrow> 'a4 set" where "set4_F' = set4_F o Rep_F'"
+definition set5_F' :: "('a1,'a2::var,'a3::var,'a4,'a5::var,'a6) F' \<Rightarrow> 'a5 set" where "set5_F' = set5_F o Rep_F'"
 
 definition asSS :: "('a \<Rightarrow> 'a) \<Rightarrow> 'a \<Rightarrow> 'a" where
   "asSS f \<equiv> if |supp f| <o |UNIV :: 'a set| then f else id"
 
-definition map_F' :: "('a1::var \<Rightarrow> 'a1) \<Rightarrow> ('a2::var \<Rightarrow> 'a2) \<Rightarrow> ('a3::var \<Rightarrow> 'a3) \<Rightarrow> ('a4 \<Rightarrow> 'a4') 
-  \<Rightarrow> ('a1,'a2,'a3,'a4) F' \<Rightarrow> ('a1,'a2,'a3,'a4') F'"
-  where "map_F' v u f g = Abs_F' o map_F (asSS v) (asSS (asBij u)) (asBij f) g o Rep_F'"
+definition map_F' :: "('a1::var \<Rightarrow> 'a1) \<Rightarrow> ('a2::var \<Rightarrow> 'a2) \<Rightarrow> ('a3::var \<Rightarrow> 'a3) \<Rightarrow> ('a4 \<Rightarrow> 'a4') \<Rightarrow> ('a5::var \<Rightarrow> 'a5)
+  \<Rightarrow> ('a1,'a2,'a3,'a4,'a5,'a6) F' \<Rightarrow> ('a1,'a2,'a3,'a4','a5,'a6) F'"
+  where "map_F' f u2 v3 g u5 = Abs_F' o map_F (asBij f) (asSS (asBij u2)) (asSS v3) g (asSS (asBij u5)) o Rep_F'"
 
-definition rrel_F' :: "('a4 \<Rightarrow> 'a4' \<Rightarrow> bool) \<Rightarrow> ('a1::var,'a2::var,'a3::var,'a4) F' \<Rightarrow> ('a1,'a2,'a3,'a4') F' \<Rightarrow> bool"
+definition rrel_F' :: "('a4 \<Rightarrow> 'a4' \<Rightarrow> bool) \<Rightarrow> ('a1,'a2::var,'a3::var,'a4,'a5::var,'a6) F' \<Rightarrow> ('a1,'a2,'a3,'a4','a5,'a6) F' \<Rightarrow> bool"
   where "rrel_F' R x x' = rrel_F (=) R (Rep_F' x) (Rep_F' x')"
 
 (* Verifying the axioms of a MRBNF for F':  *)
@@ -605,38 +481,32 @@ fun mk_map_id_tac map_F'_def F_map_id Rep_F'_inverse ctxt =
      ) ctxt)
 \<close>
 
-lemma F'_map_id: "map_F' id id id id = id"
-  apply (tactic \<open>mk_map_id_tac @{thm map_F'_def} @{thm F.map_id} @{thm Rep_F'_inverse} @{context} 
-    THEN print_tac @{context} "done" THEN no_tac\<close>)
-  apply (unfold map_F'_def asSS_def asBij_def 
-      eqTrueI[OF bij_id] eqTrueI[OF supp_id_bound] if_True)
-  apply (rule ext)
-  apply (unfold o_apply F.map_id Rep_F'_inverse)
-  apply (unfold id_def)
-  apply (rule refl)
-  done
+lemma F'_map_id: "map_F' id id id id id = id"
+  by (tactic \<open>mk_map_id_tac @{thm map_F'_def} @{thm F.map_id} @{thm Rep_F'_inverse} @{context} 
+    THEN print_tac @{context} "done"\<close>)
 
 
 ML \<open>
 open BNF_Util BNF_Tactics
 
-fun mk_map_comp_tac map_F'_def Abs_F'_inverse Rep_F' nonrep2_mapF_bij_2 F_map_comp0 ctxt =
+fun mk_map_comp_tac mrbnf map_F'_def Abs_F'_inverse Rep_F' nonrep2_mapF_bij_2 F_map_comp0 ctxt =
   HEADGOAL (Subgoal.FOCUS
-    (fn {prems = prems as [supp_u1, supp_v1, bij_u2, supp_u2, bij_v2, supp_v2, bij_u3, _, bij_v3, _],
-      context = ctxt, ...} =>
+    (fn {prems = prems, context = ctxt, ...} =>
     let
-      val _ = prems |> map @{print tracing}
-      val supp_comp = @{thm eqTrueI[OF supp_comp_bound[OF _ _ infinite_UNIV]]}
-      val bij_comp = @{thm eqTrueI[OF bij_comp]}
+      val var_types = var_types_of_mrbnf mrbnf;
+      val nr_bounds = length (filter (fn v => v = MRBNF_Def.Bound_Var) var_types);
+      val nr_frees = length (filter (fn v => v = MRBNF_Def.Free_Var) var_types);
     in
-      unfold_thms_tac ctxt ([map_F'_def,
-        supp_comp OF [supp_u1, supp_v1],
-        supp_comp OF [supp_u2, supp_v2],
-        bij_comp OF [bij_u2, bij_v2],
-        bij_comp OF [bij_u3, bij_v3]] @ map (fn thm => thm RS eqTrueI) prems @
-        @{thms asSS_def asBij_def if_True}) THEN
+      unfold_tac ctxt (map_F'_def:: @{thms asSS_def asBij_def}) THEN
+      HEADGOAL(EqSubst.eqsubst_tac ctxt (map_range (fn i => i+1) (1 + 2*nr_bounds)) @{thms bij_comp} THEN_ALL_NEW
+        TRY o resolve_tac ctxt prems) THEN
+      unfold_tac ctxt @{thms if_True} THEN
+      HEADGOAL (EqSubst.eqsubst_tac ctxt (map_range (fn i => i+1) (nr_bounds + nr_frees)) @{thms supp_comp_bound} THEN_ALL_NEW
+        TRY o resolve_tac ctxt (@{thm infinite_UNIV} ::prems)) THEN
+      unfold_tac ctxt (@{thm if_True} :: map (fn thm => thm RS eqTrueI) prems) THEN
       HEADGOAL (rtac ctxt ext) THEN
-      unfold_thms_tac ctxt [F_map_comp0 OF [supp_u1, bij_u2, supp_u2, supp_v1, bij_v2, supp_v2]] THEN
+      HEADGOAL (EqSubst.eqsubst_tac ctxt [1] [F_map_comp0] THEN_ALL_NEW
+        TRY o resolve_tac ctxt prems) THEN
       unfold_thms_tac ctxt [o_apply] THEN
       HEADGOAL (EVERY' [EqSubst.eqsubst_tac ctxt [0] [Abs_F'_inverse],
         rtac ctxt nonrep2_mapF_bij_2 THEN_ALL_NEW resolve_tac ctxt (Rep_F' :: prems),
@@ -644,36 +514,21 @@ fun mk_map_comp_tac map_F'_def Abs_F'_inverse Rep_F' nonrep2_mapF_bij_2 F_map_co
     end) ctxt)
 \<close>
 
+
 lemma F'_map_comp1_:
   fixes u1 v1 :: "'a1::var \<Rightarrow> 'a1"
   fixes u2 v2 :: "'a2::var \<Rightarrow> 'a2"
   fixes u3 v3 :: "'a3::var \<Rightarrow> 'a3"
-  assumes "|supp u1| <o |UNIV :: 'a1 set|" "|supp v1| <o |UNIV :: 'a1 set|"
+  fixes u5 v5 :: "'a5::var \<Rightarrow> 'a5"
+  assumes "bij u1" "|supp u1| <o |UNIV :: 'a1 set|" "bij v1" "|supp v1| <o |UNIV :: 'a1 set|"
   assumes "bij u2" "|supp u2| <o |UNIV :: 'a2 set|" "bij v2" "|supp v2| <o |UNIV :: 'a2 set|"
-  assumes "bij u3" "|supp u3| <o |UNIV :: 'a3 set|" "bij v3" "|supp v3| <o |UNIV :: 'a3 set|"
-  shows "map_F' (v1 o u1) (v2 o u2) (v3 o u3) (g o f) = map_F' v1 v2 v3 g o map_F' u1 u2 u3 f"
+  assumes "|supp u3| <o |UNIV :: 'a3 set|" "|supp v3| <o |UNIV :: 'a3 set|"
+  assumes "bij u5" "|supp u5| <o |UNIV :: 'a5 set|" "bij v5" "|supp v5| <o |UNIV :: 'a5 set|"
+  shows "map_F' (v1 o u1) (v2 o u2) (v3 o u3) (g o f) (v5 o u5) = map_F' v1 v2 v3 g v5 o map_F' u1 u2 u3 f u5"
   using assms apply -
-  apply (tactic \<open>mk_map_comp_tac @{thm map_F'_def} @{thm Abs_F'_inverse[unfolded mem_Collect_eq]}
+  by (tactic \<open>mk_map_comp_tac (MRBNF_Def.mrbnf_of @{context} @{type_name F} |> the) @{thm map_F'_def} @{thm Abs_F'_inverse[unfolded mem_Collect_eq]}
     @{thm Rep_F'[unfolded mem_Collect_eq]} @{thm nonrep2_mapF_bij_2} @{thm F.map_comp0} @{context} 
-    THEN print_tac @{context} "done" THEN no_tac\<close>)
-  subgoal premises prems
-    apply (unfold map_F'_def asBij_def asSS_def
-        eqTrueI[OF supp_comp_bound[OF assms(1,2) infinite_UNIV]]
-        eqTrueI[OF supp_comp_bound[OF assms(4,6) infinite_UNIV]]
-        eqTrueI[OF bij_comp[OF assms(3,5)]]
-        eqTrueI[OF bij_comp[OF assms(7,9)]]
-        eqTrueI[OF assms(5)] eqTrueI[OF assms(2)] eqTrueI[OF assms(3)] eqTrueI[OF assms(1)] eqTrueI[OF assms(4)] eqTrueI[OF assms(6)]
-        eqTrueI[OF assms(7)] eqTrueI[OF assms(9)]
-        if_True)
-    apply (rule ext)
-    apply (unfold F.map_comp0[OF assms(1,3,4,2,5,6)])
-    apply (unfold o_apply)
-    apply (subst Abs_F'_inverse[unfolded mem_Collect_eq])
-      (*apply (rule  nonrep2_mapF_bij_2[OF assms(1,3,4,7)])*)
-     apply (rule nonrep2_mapF_bij_2; (rule prems Rep_F'[unfolded mem_Collect_eq])?)
-    apply (rule refl)
-    done
-  done
+    THEN print_tac @{context} "done"\<close>)
 
 
 (* This tactic is applicable to all 4 of the following <F'_setx_map_> lemmas*)
@@ -682,135 +537,125 @@ open BNF_Util BNF_Tactics
 
 fun mk_set_map_tac set_F'_def map_F'_def Abs_F'_inverse Rep_F' nonrep2_mapF_bij_2 F_set_map ctxt =
   HEADGOAL (Subgoal.FOCUS
-    (fn {prems = prems as [supp_u1, bij_u2, supp_u2, _, _],
-      context = ctxt, ...} =>
-    let
-      val _ = prems |> map @{print tracing}
-    in
+    (fn {prems = prems, context = ctxt, ...} =>
       unfold_thms_tac ctxt ([set_F'_def, map_F'_def] @ map (fn thm => thm RS eqTrueI) prems @
         @{thms asSS_def asBij_def if_True o_apply}) THEN
       HEADGOAL (EVERY' [EqSubst.eqsubst_tac ctxt [0] [Abs_F'_inverse],
         rtac ctxt nonrep2_mapF_bij_2 THEN_ALL_NEW resolve_tac ctxt (Rep_F' :: prems),
-        rtac ctxt (F_set_map OF [supp_u1, bij_u2, supp_u2])])
-    end) ctxt)
+        rtac ctxt F_set_map THEN_ALL_NEW
+          resolve_tac ctxt prems])
+    ) ctxt)
 \<close>
 
 lemma F'_set1_map_:
   fixes u1 :: "'a1::var \<Rightarrow> 'a1"
   fixes u2 :: "'a2::var \<Rightarrow> 'a2"
   fixes u3 :: "'a3::var \<Rightarrow> 'a3"
-  assumes "|supp u1| <o |UNIV :: 'a1 set|"
+  fixes u5 :: "'a5::var \<Rightarrow> 'a5"
+  assumes "bij u1" "|supp u1| <o |UNIV :: 'a1 set|"
   assumes "bij u2" "|supp u2| <o |UNIV :: 'a2 set|"
-  assumes "bij u3" "|supp u3| <o |UNIV :: 'a3 set|"
-  shows "set1_F' (map_F' u1 u2 u3 f b) = u1 ` set1_F' b"
+  assumes "|supp u3| <o |UNIV :: 'a3 set|"
+  assumes "bij u5" "|supp u5| <o |UNIV :: 'a5 set|"
+  shows "set1_F' (map_F' u1 u2 u3 f u5 b) = u1 ` set1_F' b"
   using assms apply -
-  apply (tactic \<open>mk_set_map_tac @{thm set1_F'_def} @{thm map_F'_def} @{thm Abs_F'_inverse[unfolded mem_Collect_eq]}
+  by (tactic \<open>mk_set_map_tac @{thm set1_F'_def} @{thm map_F'_def} @{thm Abs_F'_inverse[unfolded mem_Collect_eq]}
     @{thm Rep_F'[unfolded mem_Collect_eq]} @{thm nonrep2_mapF_bij_2} @{thm F.set_map(1)} @{context} 
-    THEN print_tac @{context} "done" THEN no_tac\<close>)
-  subgoal premises prems
-    apply (unfold set1_F'_def map_F'_def asSS_def asBij_def
-        eqTrueI[OF assms(1)] eqTrueI[OF assms(2)] eqTrueI[OF assms(3)] eqTrueI[OF assms(4)] o_apply if_True)
-    apply (subst Abs_F'_inverse[unfolded mem_Collect_eq])
-      (*apply (rule nonrep2_mapF_bij_2[OF assms(1,2,3,4)])*)
-     apply (rule nonrep2_mapF_bij_2; (rule assms Rep_F'[unfolded mem_Collect_eq])?)
-    apply (rule F.set_map(1)[OF assms(1,2,3)])
-    done
-  done
+    THEN print_tac @{context} "done"\<close>)
 
 lemma F'_set2_map_:
   fixes u1 :: "'a1::var \<Rightarrow> 'a1"
   fixes u2 :: "'a2::var \<Rightarrow> 'a2"
   fixes u3 :: "'a3::var \<Rightarrow> 'a3"
-  assumes "|supp u1| <o |UNIV :: 'a1 set|"
+  fixes u5 :: "'a5::var \<Rightarrow> 'a5"
+  assumes "bij u1" "|supp u1| <o |UNIV :: 'a1 set|"
   assumes "bij u2" "|supp u2| <o |UNIV :: 'a2 set|"
-  assumes "bij u3" "|supp u3| <o |UNIV :: 'a3 set|"
-  shows "set2_F' (map_F' u1 u2 u3 f b) = u2 ` set2_F' b"
+  assumes "|supp u3| <o |UNIV :: 'a3 set|"
+  assumes "bij u5" "|supp u5| <o |UNIV :: 'a5 set|"
+  shows "set2_F' (map_F' u1 u2 u3 f u5 b) = u2 ` set2_F' b"
   using assms apply -
-  apply (tactic \<open>mk_set_map_tac @{thm set2_F'_def} @{thm map_F'_def} @{thm Abs_F'_inverse[unfolded mem_Collect_eq]}
+  by (tactic \<open>mk_set_map_tac @{thm set2_F'_def} @{thm map_F'_def} @{thm Abs_F'_inverse[unfolded mem_Collect_eq]}
     @{thm Rep_F'[unfolded mem_Collect_eq]} @{thm nonrep2_mapF_bij_2} @{thm F.set_map(2)} @{context}\<close>)
-  done
 
 lemma F'_set3_map_:
   fixes u1 :: "'a1::var \<Rightarrow> 'a1"
   fixes u2 :: "'a2::var \<Rightarrow> 'a2"
   fixes u3 :: "'a3::var \<Rightarrow> 'a3"
-  assumes "|supp u1| <o |UNIV :: 'a1 set|"
+  fixes u5 :: "'a5::var \<Rightarrow> 'a5"
+  assumes "bij u1" "|supp u1| <o |UNIV :: 'a1 set|"
   assumes "bij u2" "|supp u2| <o |UNIV :: 'a2 set|"
-  assumes "bij u3" "|supp u3| <o |UNIV :: 'a3 set|"
-  shows "set3_F' (map_F' u1 u2 u3 f b) = u3 ` set3_F' b"
+  assumes "|supp u3| <o |UNIV :: 'a3 set|"
+  assumes "bij u5" "|supp u5| <o |UNIV :: 'a5 set|"
+  shows "set3_F' (map_F' u1 u2 u3 f u5 b) = u3 ` set3_F' b"
   using assms apply -
-  apply (tactic \<open>mk_set_map_tac @{thm set3_F'_def} @{thm map_F'_def} @{thm Abs_F'_inverse[unfolded mem_Collect_eq]}
+  by (tactic \<open>mk_set_map_tac @{thm set3_F'_def} @{thm map_F'_def} @{thm Abs_F'_inverse[unfolded mem_Collect_eq]}
     @{thm Rep_F'[unfolded mem_Collect_eq]} @{thm nonrep2_mapF_bij_2} @{thm F.set_map(3)} @{context}\<close>)
-  done
 
 lemma F'_set4_map_:
   fixes u1 :: "'a1::var \<Rightarrow> 'a1"
   fixes u2 :: "'a2::var \<Rightarrow> 'a2"
   fixes u3 :: "'a3::var \<Rightarrow> 'a3"
-  assumes "|supp u1| <o |UNIV :: 'a1 set|"
+  fixes u5 :: "'a5::var \<Rightarrow> 'a5"
+  assumes "bij u1" "|supp u1| <o |UNIV :: 'a1 set|"
   assumes "bij u2" "|supp u2| <o |UNIV :: 'a2 set|"
-  assumes "bij u3" "|supp u3| <o |UNIV :: 'a3 set|"
-  shows "set4_F' (map_F' u1 u2 u3 f b) = f ` set4_F' b"
+  assumes "|supp u3| <o |UNIV :: 'a3 set|"
+  assumes "bij u5" "|supp u5| <o |UNIV :: 'a5 set|"
+  shows "set4_F' (map_F' u1 u2 u3 f u5 b) = f ` set4_F' b"
   using assms apply -
-  apply (tactic \<open>mk_set_map_tac @{thm set4_F'_def} @{thm map_F'_def} @{thm Abs_F'_inverse[unfolded mem_Collect_eq]}
+  by (tactic \<open>mk_set_map_tac @{thm set4_F'_def} @{thm map_F'_def} @{thm Abs_F'_inverse[unfolded mem_Collect_eq]}
     @{thm Rep_F'[unfolded mem_Collect_eq]} @{thm nonrep2_mapF_bij_2} @{thm F.set_map(4)} @{context}\<close>)
-  done
+
+lemma F'_set5_map_:
+  fixes u1 :: "'a1::var \<Rightarrow> 'a1"
+  fixes u2 :: "'a2::var \<Rightarrow> 'a2"
+  fixes u3 :: "'a3::var \<Rightarrow> 'a3"
+  fixes u5 :: "'a5::var \<Rightarrow> 'a5"
+  assumes "bij u1" "|supp u1| <o |UNIV :: 'a1 set|"
+  assumes "bij u2" "|supp u2| <o |UNIV :: 'a2 set|"
+  assumes "|supp u3| <o |UNIV :: 'a3 set|"
+  assumes "bij u5" "|supp u5| <o |UNIV :: 'a5 set|"
+  shows "set5_F' (map_F' u1 u2 u3 f u5 b) = u5 ` set5_F' b"
+  using assms apply -
+  by (tactic \<open>mk_set_map_tac @{thm set5_F'_def} @{thm map_F'_def} @{thm Abs_F'_inverse[unfolded mem_Collect_eq]}
+    @{thm Rep_F'[unfolded mem_Collect_eq]} @{thm nonrep2_mapF_bij_2} @{thm F.set_map(5)} @{context}\<close>)
 
 
 ML \<open>
 open BNF_Util BNF_Tactics
 
-fun mk_map_cong_tac map_F'_def set1_F'_def set2_F'_def set3_F'_def set4_F'_def  F_map_cong ctxt =
+fun mk_map_cong_tac map_F'_def F_map_cong set_F'_defs ctxt =
   HEADGOAL (Subgoal.FOCUS
-    (fn {prems = prems as [supp_u1, supp_v1, bij_u2, supp_u2, bij_v2, supp_v2, _, _, _, _,
-      eq_set1, eq_set2, eq_set3, eq_set4],
-      context = ctxt, ...} =>
-    let
-      val _ = prems |> map @{print tracing}
-    in
+    (fn {prems, context = ctxt, ...} =>
       unfold_thms_tac ctxt ([map_F'_def] @ map (fn thm => thm RS eqTrueI) prems @
         @{thms asSS_def asBij_def if_True o_apply}) THEN
-      HEADGOAL (EVERY' [
-        EqSubst.eqsubst_tac ctxt [0] [F_map_cong OF [supp_u1, bij_u2, supp_u2, supp_v1, bij_v2, supp_v2]],
-        rtac ctxt refl,
-        etac ctxt (bspec OF [unfold_thms ctxt [set1_F'_def, @{thm o_apply}] eq_set1]),
-        etac ctxt (bspec OF [unfold_thms ctxt [set2_F'_def, @{thm o_apply}] eq_set2]),
-        etac ctxt (bspec OF [unfold_thms ctxt [set3_F'_def, @{thm o_apply}] eq_set3]),
-        etac ctxt (bspec OF [unfold_thms ctxt [set4_F'_def, @{thm o_apply}] eq_set4]),
-        rtac ctxt refl])
-    end) ctxt)
+      HEADGOAL (EqSubst.eqsubst_tac ctxt [0] [F_map_cong] THEN_ALL_NEW
+        TRY o resolve_tac ctxt (rev prems)) THEN
+      HEADGOAL (rtac ctxt refl) THEN
+      REPEAT_DETERM_N (length set_F'_defs) (HEADGOAL (
+        eresolve_tac ctxt (map_index (fn (i, def) => bspec OF [unfold_thms ctxt [def, @{thm o_apply}] 
+          (nth prems (length prems - 1 - i))]) (rev set_F'_defs)))) THEN
+      HEADGOAL (rtac ctxt refl)
+    ) ctxt)
 \<close>
 
 lemma F'_map_cong_[fundef_cong]:
   fixes u1 v1 :: "'a1::var \<Rightarrow> 'a1"
   fixes u2 v2 :: "'a2::var \<Rightarrow> 'a2"
   fixes u3 v3 :: "'a3::var \<Rightarrow> 'a3"
-  assumes "|supp u1| <o |UNIV :: 'a1 set|" "|supp v1| <o |UNIV :: 'a1 set|"
+  fixes u5 v5 :: "'a5::var \<Rightarrow> 'a5"
+  assumes "bij u1" "|supp u1| <o |UNIV :: 'a1 set|" "bij v1" "|supp v1| <o |UNIV :: 'a1 set|"
   assumes "bij u2" "|supp u2| <o |UNIV :: 'a2 set|" "bij v2" "|supp v2| <o |UNIV :: 'a2 set|"
-  assumes "bij u3" "|supp u3| <o |UNIV :: 'a3 set|" "bij v3" "|supp v3| <o |UNIV :: 'a3 set|"
+  assumes "|supp u3| <o |UNIV :: 'a3 set|" "|supp v3| <o |UNIV :: 'a3 set|"
+  assumes "bij u5" "|supp u5| <o |UNIV :: 'a5 set|" "bij v5" "|supp v5| <o |UNIV :: 'a5 set|"
     and "\<forall> a \<in> set1_F' x. u1 a = v1 a"
     and "\<forall> a \<in> set2_F' x. u2 a = v2 a"
     and "\<forall> a \<in> set3_F' x. u3 a = v3 a"
     and "\<forall> a \<in> set4_F' x. f a = g a"
-  shows "map_F' u1 u2 u3 f x = map_F' v1 v2 v3 g x"
+    and "\<forall> a \<in> set5_F' x. u5 a = v5 a"
+  shows "map_F' u1 u2 u3 f u5 x = map_F' v1 v2 v3 g v5 x"
   using assms apply -
-  apply (tactic \<open>mk_map_cong_tac @{thm map_F'_def} @{thm set1_F'_def} @{thm set2_F'_def} 
-    @{thm set3_F'_def} @{thm set4_F'_def} @{thm F.map_cong} @{context} 
-    THEN print_tac @{context} "done" THEN no_tac\<close>)
-  subgoal premises prems
-    apply (unfold map_F'_def asSS_def asBij_def 
-        eqTrueI[OF assms(1)] eqTrueI[OF assms(2)] eqTrueI[OF assms(3)] eqTrueI[OF assms(4)] eqTrueI[OF assms(5)] 
-        eqTrueI[OF assms(6)] eqTrueI[OF assms(7)] eqTrueI[OF assms(9)] if_True o_apply)
-    apply (subst F.map_cong[OF prems(1,3,4,2,5,6)])
-         apply (rule refl)
-        apply (erule bspec[OF prems(11)[unfolded set1_F'_def o_apply]])
-       apply (erule bspec[OF prems(12)[unfolded set2_F'_def o_apply]])
-      apply (erule bspec[OF prems(13)[unfolded set3_F'_def o_apply]])
-     apply (erule bspec[OF prems(14)[unfolded set4_F'_def o_apply]])
-    apply (rule refl)
-    done
-  done
-
+  by (tactic \<open>mk_map_cong_tac @{thm map_F'_def} @{thm F.map_cong} 
+    @{thms set1_F'_def set2_F'_def set3_F'_def set4_F'_def set5_F'_def} @{context} 
+    THEN print_tac @{context} "done"\<close>)
 
 (* This tactic is applicable to all 4 of the following <F'_setx_bd> lemmas*)
 ML \<open>
@@ -822,131 +667,105 @@ fun mk_set_bd_tac set_F'_def F_set_bd ctxt =
 \<close>
 
 lemma F'_set1_bd: "\<And>b. |set1_F' b| <o natLeq"
-  apply (tactic \<open>mk_set_bd_tac @{thm set1_F'_def} @{thm F.set_bd(1)} @{context}
-    THEN print_tac @{context} "done" THEN no_tac\<close>)
-  apply (unfold set1_F'_def o_apply)
-  apply (rule F.set_bd(1))
-  done
+  by (tactic \<open>mk_set_bd_tac @{thm set1_F'_def} @{thm F.set_bd(1)} @{context}\<close>)
 lemma F'_set2_bd: "\<And>b. |set2_F' b| <o natLeq"
-  apply (tactic \<open>mk_set_bd_tac @{thm set2_F'_def} @{thm F.set_bd(2)} @{context}\<close>)
-  done
+  by (tactic \<open>mk_set_bd_tac @{thm set2_F'_def} @{thm F.set_bd(2)} @{context}\<close>)
 lemma F'_set3_bd: "\<And>b. |set3_F' b| <o natLeq"
-  apply (tactic \<open>mk_set_bd_tac @{thm set3_F'_def} @{thm F.set_bd(3)} @{context}\<close>)
-  done
+  by (tactic \<open>mk_set_bd_tac @{thm set3_F'_def} @{thm F.set_bd(3)} @{context}\<close>)
 lemma F'_set4_bd: "\<And>b. |set4_F' b| <o natLeq"
-  apply (tactic \<open>mk_set_bd_tac @{thm set4_F'_def} @{thm F.set_bd(4)} @{context}\<close>)
-  done
+  by (tactic \<open>mk_set_bd_tac @{thm set4_F'_def} @{thm F.set_bd(4)} @{context}\<close>)
 
 ML \<open>
 open BNF_Util BNF_Tactics
 
 fun mk_rel_comp_leq_tac rrel_F'_def F_rel_compp ctxt =
- HEADGOAL (Subgoal.FOCUS
-    (fn {context = ctxt, ...} => print_tac @{context} "0" THEN
-      HEADGOAL (rtac ctxt @{thm predicate2I}) THEN print_tac @{context} "1" THEN
-      HEADGOAL (etac ctxt @{thm relcomppE}) THEN print_tac @{context} "2" THEN
-      unfold_thms_tac ctxt [rrel_F'_def] THEN print_tac @{context} "3" THEN
-      HEADGOAL (EqSubst.eqsubst_tac ctxt [1] (@{thms eq_OO[symmetric]})) THEN print_tac @{context} "4" THEN
-      HEADGOAL (EqSubst.eqsubst_tac ctxt [1] ([F_rel_compp])) THEN print_tac @{context} "5" THEN
-      unfold_thms_tac ctxt [rrel_F'_def] THEN print_tac @{context} "6" THEN
-      HEADGOAL (rtac ctxt @{thm relcomppI} THEN_ALL_NEW assume_tac ctxt)
-    ) ctxt)
-  
+  HEADGOAL (EVERY' [
+    rtac ctxt @{thm predicate2I},
+    etac ctxt @{thm relcomppE},
+    K (unfold_tac ctxt [rrel_F'_def]),
+    EqSubst.eqsubst_tac ctxt [1] (@{thms eq_OO[symmetric]}),
+    EqSubst.eqsubst_tac ctxt [1] ([F_rel_compp]),
+    K (unfold_tac ctxt [rrel_F'_def]),
+    rtac ctxt @{thm relcomppI} THEN_ALL_NEW assume_tac ctxt
+  ])
 \<close>
 
 lemma F'_rel_comp_leq_: "rrel_F' Q OO rrel_F' R \<le> rrel_F' (Q OO R)"
-  apply (tactic \<open>mk_rel_comp_leq_tac @{thm rrel_F'_def} @{thm F.rel_compp} @{context}
-    THEN print_tac @{context} "done" THEN no_tac\<close>)
-  subgoal premises prems
-    apply (rule predicate2I)
-    apply (erule relcomppE)
-    apply (unfold rrel_F'_def) (* Somehow this only unfolds the goal in the tactic *)
-    apply (subst (1) eq_OO[symmetric])
-    apply (subst (1) F.rel_compp)
-      (*apply (unfold rrel_F'_def)*)
-    apply (rule relcomppI; (assumption))
-    done
-  done
+  by (tactic \<open>mk_rel_comp_leq_tac @{thm rrel_F'_def} @{thm F.rel_compp} @{context}
+    THEN print_tac @{context} "done"\<close>)
 
 ML \<open>
 open BNF_Util BNF_Tactics
 
 fun mk_rrel_F_map_F3_tac F_rel_map F_rel_mono_strong Grp_def ctxt =
-  HEADGOAL (Subgoal.FOCUS
-    (fn {context = ctxt, ...} =>
-      unfold_thms_tac ctxt ([F_rel_map, Grp_def, eqTrueI OF @{thms UNIV_I}] @ @{thms id_apply simp_thms(21)}) THEN
-      HEADGOAL (rtac ctxt @{thm iffI}) THEN
-      ALLGOALS (EVERY' [etac ctxt F_rel_mono_strong, etac ctxt sym, assume_tac ctxt])
-    ) ctxt)
+    unfold_thms_tac ctxt ([F_rel_map, Grp_def, eqTrueI OF @{thms UNIV_I}] @ @{thms id_apply simp_thms(21)}) THEN
+    HEADGOAL (rtac ctxt @{thm iffI}) THEN
+    ALLGOALS (EVERY' [etac ctxt F_rel_mono_strong, etac ctxt sym, assume_tac ctxt])
 \<close>
 
 lemma rrel_F_map_F3:
-  fixes x :: "('a :: var,'b :: var,'c,'d) F"
-  shows "rrel_F (Grp (f :: 'c \<Rightarrow> 'c)) R x y = rrel_F (=) R (map_F id id f id x) y"
-  apply (tactic \<open>mk_rrel_F_map_F3_tac @{thm F.rel_map(1)} @{thm F.rel_mono_strong} @{thm Grp_def} @{context} 
-    THEN print_tac @{context} "done" THEN no_tac\<close>)
-  subgoal premises prems
-    apply (unfold F.rel_map(1) Grp_def id_apply eqTrueI[OF UNIV_I] simp_thms(21))
-    apply (rule iffI)
-     apply (erule F.rel_mono_strong, erule sym, assumption)+
-    done
-  done
-
+  fixes x :: "('a,'b::var,'c::var,'d,'e::var,'f) F"
+  shows "rrel_F (Grp (f :: 'a \<Rightarrow> 'a)) R x y = rrel_F (=) R (map_F f id id id id x) y"
+  by (tactic \<open>mk_rrel_F_map_F3_tac @{thm F.rel_map(1)} @{thm F.rel_mono_strong} @{thm Grp_def} @{context} 
+    THEN print_tac @{context} "done"\<close>)
 
 ML \<open>
 open BNF_Util BNF_Tactics
 
 fun mk_asSS_tac ctxt =
-  HEADGOAL (Subgoal.FOCUS
-    (fn {prems, context = ctxt, ...} =>
-      unfold_thms_tac ctxt @{thms asSS_def} THEN
-      HEADGOAL (rtac ctxt @{thm if_P}) THEN
-      HEADGOAL (rtac ctxt (nth prems 0))
-    ) ctxt)
+  unfold_thms_tac ctxt @{thms asSS_def} THEN
+  HEADGOAL (rtac ctxt @{thm if_P}) THEN
+  HEADGOAL (assume_tac ctxt)
 \<close>
 
 lemma asSS: "|supp u| <o |UNIV :: 'a set| \<Longrightarrow> asSS (u :: 'a \<Rightarrow> 'a) = u"
-  apply (tactic \<open>mk_asSS_tac @{context} 
-    THEN print_tac @{context} "done" THEN no_tac\<close>)
-  subgoal premises prems
-    apply (unfold asSS_def)
-    apply (rule if_P) 
-    apply (rule prems)
-    done
-  done
+  by (tactic \<open>mk_asSS_tac @{context} 
+    THEN print_tac @{context} "done"\<close>)
 
 ML \<open>
-open BNF_Util BNF_Tactics
+open BNF_Util BNF_Tactics MRBNF_Def
 
-fun mk_in_rel_tac rrel_F'_def set4_F'_def map_F'_def Abs_F'_inverse Rep_F' nonrep2_mapF_bij_2 
-  rrel_F_map_F3 F_in_rel F_map_comp nonrep2_map_F_rev F_set_map3 F_set_map4 Rep_F'_inverse F_map_cong cx ctxt =
+fun mk_in_rel_tac mrbnf rrel_F'_def set4_F'_def map_F'_def Abs_F'_inverse Rep_F' nonrep2_mapF_bij_2 
+  rrel_F_map_F3 F_in_rel F_map_comp nonrep2_map_F_rev Rep_F'_inverse F_map_cong F_set_maps cx ctxt =
   HEADGOAL (Subgoal.FOCUS
     (fn {prems, context = ctxt,...} =>
+      let
+        fun mk_sb_prems _ [] _ = []
+        | mk_sb_prems prems (Live_Var::vars) i = if i = lin_pos then (mk_sb_prems (drop 2 prems) vars (i+1)) else (mk_sb_prems prems vars (i+1))
+        | mk_sb_prems (bp::sp::prems) (Bound_Var::vars) i = bp::sp::(mk_sb_prems prems vars (i+1))
+        | mk_sb_prems (sp::prems) (Free_Var::vars) i = sp::(mk_sb_prems prems vars (i+1))
+        | mk_sb_prems prems (Dead_Var::vars) i = (mk_sb_prems prems vars (i+1))
+        | mk_sb_prems _ _ _ = [];
+
+        val var_types = var_types_of_mrbnf mrbnf;
+        val id_prems = MRBNF_Comp_Tactics.mk_id_prems mrbnf;
+        val sb_prems = mk_sb_prems prems var_types 1;
+        val nr_lives = length (filter (fn v => v = Live_Var) var_types);
+      in
         unfold_thms_tac ctxt ([rrel_F'_def, set4_F'_def, map_F'_def, o_apply] @ @{thms asSS_def asBij_def if_True} @ 
           map (fn thm => thm RS eqTrueI) (prems @ @{thms supp_id_bound bij_id})) THEN
         HEADGOAL (EqSubst.eqsubst_tac ctxt [0] [Abs_F'_inverse])THEN
         HEADGOAL (rtac ctxt nonrep2_mapF_bij_2 THEN_ALL_NEW resolve_tac ctxt (Rep_F' :: prems)) THEN
-        HEADGOAL (EqSubst.eqsubst_tac ctxt [0] [(unfold_thms ctxt ((F_map_comp OF ((take 3 prems) @ @{thms supp_id_bound bij_id supp_id_bound})):: @{thms id_o o_id})
-          (trans OF [rrel_F_map_F3 RS sym, F_in_rel OF (take 3 prems)]))]) THEN
+        HEADGOAL (EqSubst.eqsubst_tac ctxt [0] [(unfold_thms ctxt ((F_map_comp OF (sb_prems @ id_prems)):: @{thms id_o o_id})
+          (trans OF [rrel_F_map_F3 RS sym, F_in_rel OF sb_prems]))]) THEN
         unfold_thms_tac ctxt ((eqTrueI OF @{thms UNIV_I}):: @{thms Grp_def simp_thms(21)}) THEN
         HEADGOAL (rtac ctxt iffI) THEN
         (* 1st Subgoal *)
         REPEAT_DETERM_N 5 (HEADGOAL (eresolve_tac ctxt [exE, conjE, CollectE])) THEN
         HEADGOAL (Subgoal.FOCUS
-          (fn {prems = subprems, context = ctxt, params, ...} =>
-            let
-              val _ = subprems |> map @{print tracing};
-              val _ = params |> map @{print tracing};
-            in
+          (fn {prems = subprems, context = ctxt, ...} =>
               (* setup *)
               HEADGOAL (EVERY' [
                 rtac ctxt exI,
                 EqSubst.eqsubst_tac ctxt [1, 2, 3] [Abs_F'_inverse],
                 Method.insert_tac ctxt [unfold_thms ctxt [(nth subprems 0 RS sym)] (infer_instantiate' ctxt [SOME cx] Rep_F')],
-                EqSubst.eqsubst_asm_tac ctxt [8] [@{thm id_o} RS sym],
-                EqSubst.eqsubst_asm_tac ctxt [4, 6, 14] [@{thm o_id} RS sym],
-                EqSubst.eqsubst_asm_tac ctxt [0] [F_map_comp OF @{thms supp_id_bound bij_id supp_id_bound supp_id_bound bij_id supp_id_bound} RS sym],
-                dtac ctxt (nonrep2_map_F_rev OF @{thms bij_id supp_id_bound}),
+                EqSubst.eqsubst_asm_tac ctxt (map_range (fn i => if i < lin_pos-1 then 4+2*i else 4+2*(i+1)) (length var_types-1)) 
+                  [@{thm o_id} RS sym],
+                EqSubst.eqsubst_asm_tac ctxt [4+6*(lin_pos-1)] [@{thm id_o} RS sym],
+                EqSubst.eqsubst_asm_tac ctxt [0] [F_map_comp RS sym] THEN_ALL_NEW
+                  TRY o resolve_tac ctxt @{thms bij_id supp_id_bound},
+                dtac ctxt (rotate_prems ~1 nonrep2_map_F_rev) THEN_ALL_NEW
+                  TRY o resolve_tac ctxt @{thms bij_id supp_id_bound},
                 assume_tac ctxt
               ]) THEN
               (* solve *)
@@ -955,7 +774,8 @@ fun mk_in_rel_tac rrel_F'_def set4_F'_def map_F'_def Abs_F'_inverse Rep_F' nonre
                   TRY o resolve_tac ctxt (prems @ @{thms bij_id supp_id_bound}),
                 K (unfold_thms_tac ctxt @{thms id_o o_id}),
                 rtac ctxt conjI,
-                EqSubst.eqsubst_tac ctxt [0] [F_set_map4 OF @{thms supp_id_bound bij_id supp_id_bound}],
+                EqSubst.eqsubst_tac ctxt [0] F_set_maps THEN_ALL_NEW (*something has to be repeated forall non-lin_pos lives*)
+                  TRY o resolve_tac ctxt @{thms bij_id supp_id_bound},
                 EqSubst.eqsubst_tac ctxt [0] @{thms image_id},
                 resolve_tac ctxt subprems,
                 EqSubst.eqsubst_tac ctxt [2, 4] [Rep_F'_inverse RS sym],
@@ -970,59 +790,58 @@ fun mk_in_rel_tac rrel_F'_def set4_F'_def map_F'_def Abs_F'_inverse Rep_F' nonre
                 EqSubst.eqsubst_tac ctxt [0] [o_apply],
                 assume_tac ctxt
               ])
-            end) 
+            ) 
           ctxt) THEN
         (* 2nd Subgoal *)
         REPEAT_DETERM_N 3 (HEADGOAL (eresolve_tac ctxt [exE, conjE])) THEN
         HEADGOAL (hyp_subst_tac_thin true ctxt) THEN
         HEADGOAL (Subgoal.FOCUS
           (fn {prems = subprems, context = ctxt, ...} =>
-            let
-              val _ = subprems |> map @{print tracing};
-            in
-              HEADGOAL (EVERY' [
-                rtac ctxt exI,
-                EqSubst.eqsubst_tac ctxt [0] [Abs_F'_inverse],
-                rtac ctxt nonrep2_mapF_bij_2 THEN_ALL_NEW
-                  TRY o resolve_tac ctxt (Rep_F':: @{thms supp_id_bound bij_id}),
-                rtac ctxt conjI THEN_ALL_NEW TRY o rtac ctxt conjI 
-              ]) THEN
-              prefer_tac 3 THEN
-              HEADGOAL (EVERY' [
-                EqSubst.eqsubst_tac ctxt [0] [Abs_F'_inverse],
-                rtac ctxt nonrep2_mapF_bij_2 THEN_ALL_NEW                
-                  TRY o resolve_tac ctxt (Rep_F':: prems),
-                EqSubst.eqsubst_tac ctxt [0] [F_map_comp OF @{thms supp_id_bound bij_id supp_id_bound}] THEN_ALL_NEW
-                  TRY o resolve_tac ctxt prems,
-                K (unfold_thms_tac ctxt @{thms o_id}),
-                EqSubst.eqsubst_tac ctxt [1, 2] @{thms o_def},
-                rtac ctxt F_map_cong THEN_ALL_NEW
-                  TRY o resolve_tac ctxt (refl::prems),
-                rtac ctxt @{thm snd_conv},
-                rtac ctxt CollectI,
-                EqSubst.eqsubst_tac ctxt [0] [F_set_map3 OF @{thms supp_id_bound bij_id supp_id_bound}],
-                EqSubst.eqsubst_tac ctxt [0] [F_set_map4 OF @{thms supp_id_bound bij_id supp_id_bound}],
-                EqSubst.eqsubst_tac ctxt [0] @{thms image_ident},
-                rtac ctxt conjI,
-                rtac ctxt subsetI,
-                etac ctxt imageE,
-                rtac ctxt CollectI,
-                rtac ctxt @{thm case_prodI2},
-                dtac ctxt (trans OF [sym] RS (iffD1 OF @{thms prod.inject})),
-                assume_tac ctxt,
-                etac ctxt conjE,
-                rtac ctxt (trans OF [sym]),
-                assume_tac ctxt,
-                etac ctxt arg_cong,
-                resolve_tac ctxt subprems,
-                EqSubst.eqsubst_tac ctxt [0] [F_map_comp] THEN_ALL_NEW
-                  TRY o resolve_tac ctxt @{thms supp_id_bound bij_id},
-                K (unfold_thms_tac ctxt @{thms o_def id_def fst_conv}),
-                rtac ctxt refl
-              ])
-            end) 
+            HEADGOAL (EVERY' [
+              rtac ctxt exI,
+              EqSubst.eqsubst_tac ctxt [0] [Abs_F'_inverse],
+              rtac ctxt nonrep2_mapF_bij_2 THEN_ALL_NEW
+                TRY o resolve_tac ctxt (Rep_F':: @{thms supp_id_bound bij_id}),
+              rtac ctxt conjI THEN_ALL_NEW TRY o rtac ctxt conjI 
+            ]) THEN
+            prefer_tac 3 THEN
+            HEADGOAL (EVERY' [
+              EqSubst.eqsubst_tac ctxt [0] [Abs_F'_inverse],
+              rtac ctxt nonrep2_mapF_bij_2 THEN_ALL_NEW                
+                TRY o resolve_tac ctxt (Rep_F':: prems),
+              EqSubst.eqsubst_tac ctxt [0] [F_map_comp] THEN_ALL_NEW
+                TRY o resolve_tac ctxt (@{thms bij_id supp_id_bound} @ prems),
+              K (unfold_thms_tac ctxt @{thms o_id}),
+              EqSubst.eqsubst_tac ctxt [1, 2] @{thms o_def},
+              rtac ctxt F_map_cong THEN_ALL_NEW
+                TRY o resolve_tac ctxt (refl::prems),
+              rtac ctxt @{thm snd_conv},
+              rtac ctxt CollectI
+            ]) THEN
+            REPEAT_DETERM_N (nr_lives) (
+              HEADGOAL (EqSubst.eqsubst_tac ctxt [0] F_set_maps THEN_ALL_NEW
+                TRY o resolve_tac ctxt @{thms bij_id supp_id_bound})) THEN
+            HEADGOAL (EVERY' [
+              EqSubst.eqsubst_tac ctxt [0] @{thms image_ident},
+              rtac ctxt conjI,
+              rtac ctxt subsetI,
+              etac ctxt imageE,
+              rtac ctxt CollectI,
+              rtac ctxt @{thm case_prodI2},
+              dtac ctxt (trans OF [sym] RS (iffD1 OF @{thms prod.inject})),
+              assume_tac ctxt,
+              etac ctxt conjE,
+              rtac ctxt (trans OF [sym]),
+              assume_tac ctxt,
+              etac ctxt arg_cong,
+              resolve_tac ctxt subprems,
+              EqSubst.eqsubst_tac ctxt [0] [F_map_comp] THEN_ALL_NEW
+                TRY o resolve_tac ctxt @{thms supp_id_bound bij_id},
+              K (unfold_thms_tac ctxt @{thms o_def id_def fst_conv}),
+              rtac ctxt refl
+            ])) 
           ctxt) 
-    ) ctxt)
+    end) ctxt)
 \<close>
 
 
@@ -1030,128 +849,20 @@ lemma F'_in_rel:
   fixes u1 :: "'a1::var \<Rightarrow> 'a1"
   fixes u2 :: "'a2::var \<Rightarrow> 'a2"
   fixes u3 :: "'a3::var \<Rightarrow> 'a3"
-  assumes u1: "|supp u1| <o |UNIV :: 'a1 set|"
+  fixes u5 :: "'a5::var \<Rightarrow> 'a5"
+  assumes u1: "bij u1" "|supp u1| <o |UNIV :: 'a1 set|"
     and u2: "bij u2" "|supp u2| <o |UNIV :: 'a2 set|" 
-    and u3: "bij u3" "|supp u3| <o |UNIV :: 'a3 set|"
-  shows "rrel_F' R (map_F' u1 u2 u3 id x) y =
-    (\<exists>z. set4_F' z \<subseteq> {(x, y). R x y} \<and> map_F' id id id fst z = x \<and> map_F' u1 u2 u3 snd z = y)"
+    and u3: "|supp u3| <o |UNIV :: 'a3 set|"
+    and u5: "bij u5" "|supp u5| <o |UNIV :: 'a5 set|"
+  shows "rrel_F' R (map_F' u1 u2 u3 id u5 x) y =
+    (\<exists>z. set4_F' z \<subseteq> {(x, y). R x y} \<and> map_F' id id id fst id z = x \<and> map_F' u1 u2 u3 snd u5 z = y)"
   using assms apply -
-  apply (tactic \<open>mk_in_rel_tac @{thm rrel_F'_def} @{thm set4_F'_def} @{thm map_F'_def} @{thm Abs_F'_inverse[unfolded mem_Collect_eq]}
+  by (tactic \<open>mk_in_rel_tac (MRBNF_Def.mrbnf_of @{context} @{type_name F} |> the) @{thm rrel_F'_def} 
+    @{thm set4_F'_def} @{thm map_F'_def} @{thm Abs_F'_inverse[unfolded mem_Collect_eq]}
     @{thm Rep_F'[unfolded mem_Collect_eq]} @{thm nonrep2_mapF_bij_2} @{thm rrel_F_map_F3} @{thm F.in_rel}
-    @{thm F.map_comp} @{thm nonrep2_map_F_rev} @{thm F.set_map(3)} @{thm F.set_map(4)} @{thm Rep_F'_inverse} @{thm F.map_cong}
+    @{thm F.map_comp} @{thm nonrep2_map_F_rev} @{thm Rep_F'_inverse} @{thm F.map_cong} @{thms F.set_map}
     @{cterm x} @{context}
-    THEN print_tac @{context} "done" THEN no_tac\<close>)
-  subgoal premises prems
-    apply (unfold rrel_F'_def set4_F'_def map_F'_def asSS_def asBij_def if_True 
-        eqTrueI[OF prems(1)] eqTrueI[OF prems(2)] eqTrueI[OF prems(3)] eqTrueI[OF prems(4)] 
-        eqTrueI[OF supp_id_bound] eqTrueI[OF bij_id] o_apply)
-    apply (subst Abs_F'_inverse[unfolded mem_Collect_eq])
-     apply (rule nonrep2_mapF_bij_2; (rule prems Rep_F'[unfolded mem_Collect_eq])?)
-    apply (subst trans[OF rrel_F_map_F3[symmetric] F.in_rel[OF prems(1,2,3)],
-          unfolded F.map_comp[OF prems(1,2,3) supp_id_bound bij_id supp_id_bound] id_o o_id])
-    apply (unfold Grp_def eqTrueI[OF UNIV_I] simp_thms(21))
-    apply (rule iffI)
-     apply (erule exE)
-     apply (erule conjE)
-     apply (erule conjE)
-     apply (erule CollectE)
-     apply (erule conjE)
-    subgoal premises subprems for z
-      (*     apply (tactic \<open>
-        let
-          val ctxt = @{context};
-          val cz = @{cterm z};
-          val z = Thm.term_of cz;
-          val zT = fastype_of z;
-          val which = 0;
-          val Abs_F' = @{term Abs_F'}
-          val mrbnf = MRBNF_Def.mrbnf_of ctxt @{type_name F} |> the;
-          val subst = Sign.typ_match (Proof_Context.theory_of ctxt)
-            (MRBNF_Def.T_of_mrbnf mrbnf, zT) Vartab.empty;
-          val deads = MRBNF_Def.deads_of_mrbnf mrbnf |> map (Envir.subst_type subst) |> @{print};
-          val frees = MRBNF_Def.frees_of_mrbnf mrbnf |> map (Envir.subst_type subst) |> @{print};
-          val bounds = MRBNF_Def.bounds_of_mrbnf mrbnf |> map (Envir.subst_type subst) |> @{print};
-          val lives = MRBNF_Def.lives_of_mrbnf mrbnf |> map (Envir.subst_type subst) |> @{print};
-          val map_F = MRBNF_Def.mk_map_comb_of_mrbnf deads
-            (map_index (uncurry (fn i => if i = which then BNF_Util.fst_const else HOLogic.id_const)) lives)
-            (map HOLogic.id_const bounds) (map HOLogic.id_const frees)
-            mrbnf $ z |> @{print};
-          val Ts = fastype_of map_F |> dest_Type |> snd;
-          val Us = domain_type (fastype_of Abs_F') |> dest_Type |> snd;
-          val ct = Thm.cterm_of ctxt (subst_atomic_types (Us ~~ Ts) Abs_F' $ map_F) |> @{print};
-        in
-          HEADGOAL (BNF_Util.rtac ctxt (infer_instantiate' ctxt [NONE, SOME ct] exI))
-        end
-        \<close>) *)
-      apply (rule exI)
-      apply (subst (1 2 3) Abs_F'_inverse[unfolded mem_Collect_eq])
-       apply (insert Rep_F'[of x, unfolded mem_Collect_eq subprems(1)[symmetric]]) []
-       apply (subst (asm) (8) id_o[symmetric])
-       apply (subst (asm) (4 6 14) o_id[symmetric])
-       apply (subst (asm) F.map_comp[OF supp_id_bound bij_id supp_id_bound supp_id_bound bij_id supp_id_bound, symmetric])
-       apply (drule nonrep2_map_F_rev[OF bij_id supp_id_bound])
-       apply (assumption)
-
-      apply (subst (1 2) F.map_comp; (rule supp_id_bound bij_id prems(1,2,3))?)
-      apply (unfold o_id id_o)
-      apply (rule conjI)
-       apply (subst F.set_map(4)[OF supp_id_bound bij_id supp_id_bound])
-       apply (subst image_id)
-       apply (rule subprems)
-      apply (subst (2 4) Rep_F'_inverse[symmetric])
-      apply (rule conjI)
-       apply (rule arg_cong[OF subprems(1)])
-      apply (subst subprems(2)[symmetric])
-      apply (rule F.map_cong[THEN arg_cong]; (rule prems refl)?)
-      apply (drule rev_subsetD[THEN Collect_case_prodD])
-       apply (rule subprems)
-      apply (rule sym)
-      apply (subst o_apply)
-      apply (assumption)
-      done
-    apply (erule exE)
-    apply (erule conjE)
-    apply (erule conjE)
-    apply (hypsubst_thin)
-    subgoal premises subprems for z
-      apply (rule exI)
-      apply (subst Abs_F'_inverse[unfolded mem_Collect_eq])
-       apply (rule nonrep2_mapF_bij_2; (rule supp_id_bound bij_id Rep_F'[unfolded mem_Collect_eq])?)
-      apply (rule conjI; (rule conjI)?)
-
-        prefer 3(* subgoal 3 is solvable without the exI instantiation and it transforms "?z" 
-          so that the other 2 subgoals are solvable as well*)
-        apply (subst Abs_F'_inverse[unfolded mem_Collect_eq])
-         apply (rule nonrep2_mapF_bij_2; (rule prems Rep_F'[unfolded mem_Collect_eq])?)
-        apply (subst F.map_comp[OF supp_id_bound bij_id supp_id_bound]; (rule prems(1,2,3))?)
-        apply (unfold o_id)
-        apply (subst (1 2) o_def)
-        apply (rule F.map_cong; (rule prems(1,2,3) refl)?)
-        apply (rule snd_conv)
-
-       apply (rule CollectI)
-       apply (subst F.set_map(3)[OF supp_id_bound bij_id supp_id_bound])
-       apply (subst F.set_map(4)[OF supp_id_bound bij_id supp_id_bound])
-       apply (subst image_ident)
-       apply (rule conjI) 
-        apply (rule subsetI)
-        apply (erule imageE)
-        apply (rule CollectI)
-        apply (rule case_prodI2)
-        apply (drule trans[OF sym, THEN iffD1[OF prod.inject]])
-         apply (assumption)
-        apply (erule conjE)
-        apply (rule trans[OF sym])
-         apply (assumption)
-        apply (erule arg_cong) 
-       apply (rule subprems)
-
-      apply (subst F.map_comp; (rule supp_id_bound bij_id)?)
-      apply (unfold o_def fst_conv id_def)
-      apply (rule refl)
-      done
-    done
-  done
+    THEN print_tac @{context} "done"\<close>)
 
 ML \<open>
 open BNF_Util BNF_Tactics
@@ -1159,14 +870,11 @@ open BNF_Util BNF_Tactics
 fun mk_strong_tac rrel_F'_def mr_rel_F_def F_strong F_map_id ctxt =
   HEADGOAL (Subgoal.FOCUS
     (fn {prems, context = ctxt, ...} => 
-    let
-      val _ = prems |> map @{print tracing}
-    in
       unfold_thms_tac ctxt [rrel_F'_def] THEN
       HEADGOAL (rtac ctxt (unfold_thms ctxt @{thms inf.idem} 
         (unfold_thms ctxt [mr_rel_F_def, F_map_id] F_strong
          OF (map (fn prem => unfold_thms ctxt [rrel_F'_def] prem) prems))))
-    end) ctxt)
+    ) ctxt)
 \<close>
 
 lemma F'_strong:
@@ -1174,15 +882,8 @@ lemma F'_strong:
     and "rrel_F' Q x x'"
   shows "rrel_F' (inf R Q) x x'" 
   using assms apply -
-  apply (tactic \<open>mk_strong_tac @{thm rrel_F'_def} @{thm mr_rel_F_def} @{thm F_strong} @{thm F.map_id} @{context} 
-    THEN print_tac @{context} "done" THEN no_tac\<close>)
-  subgoal premises prems
-    apply (unfold rrel_F'_def)
-    apply (rule F_strong[unfolded mr_rel_F_def F.map_id, 
-          OF prems(1)[unfolded rrel_F'_def] prems(2)[unfolded rrel_F'_def], 
-          unfolded inf.idem])
-    done
-  done
+  by (tactic \<open>mk_strong_tac @{thm rrel_F'_def} @{thm mr_rel_F_def} @{thm F_strong} @{thm F.map_id} @{context} 
+    THEN print_tac @{context} "done"\<close>)
 
 ML \<open>
 open BNF_Util BNF_Tactics
@@ -1218,9 +919,9 @@ fun mk_is_mrbnf_tac F'_map_id F'_map_comp1 F'_map_cong F'_set1_map F'_set2_map F
 
 
 
-mrbnf "('a::var, 'b::var, 'c::var, 'd) F'"
+mrbnf "('a, 'b :: var, 'c :: var, 'd, 'e :: var, 'f) F'"
   map: map_F'
-  sets: free: set1_F' bound: set2_F' bound: set3_F' live: set4_F'
+  sets: live: set1_F' bound: set2_F' free: set3_F' live: set4_F' bound: set5_F'
   bd: natLeq
   rel: rrel_F'
   var_class: var
